CCDeconstructed/Env.lean
@@ -1,84 +1,378 @@
+import CCDeconstructed.CC
 import CCDeconstructed.Var
 import CCDeconstructed.Syntax
-import CCDeconstructed.CC
 
-import Mathlib.Data.Finset.Fold
-import Mathlib.Data.List.Nodup
 import Mathlib.Data.List.AList
 
-open Feature VarCat
+set_option linter.unusedVariables false
 
-inductive Binding : VarCat i -> Type :=
-  | val : Typ i -> Binding (var i)
-  | sub : Typ i -> Binding (tvar i)
-  | typ [HasFeature i type_bindings] : Typ i -> Binding (tvar i)
+open VarCat Feature
+
+namespace AList
+  lemma insert_erase.{u}
+    {α : Type u} {β : α → Type} [DecidableEq α]
+    {a a' : α} (s : AList β) (b : β a) :
+    a ≠ a' →
+    AList.insert a b (AList.erase a' s) =
+    AList.erase a' (AList.insert a b s)
+  := by
+    intros Neq
+    simp [AList.insert,AList.erase]
+    rw [List.kerase_cons_ne (Neq ∘ Eq.symm)]
+    congr 1
+    apply List.kerase_kerase
+
+  lemma erase_of_not_mem.{u, v} {α : Type u} {β : α → Type v} [DecidableEq α] {a : α} {s : AList β} :
+    a ∉ s →
+    AList.erase a s = s
+  := by
+    intros NotIn
+    obtain ⟨entries,nodupKeys⟩ := s
+    induction entries
+    · case nil => simp [AList.erase]
+    · case cons b s.entries IH =>
+      simp [AList.erase,List.kerase,List.eraseP]
+      split
+      · case inl eq =>
+        exfalso
+        apply NotIn
+        simp [Membership.mem,AList.keys]
+        rw [eq]
+        apply List.Mem.head
+      · case inr neq =>
+        simp [AList.erase,List.kerase] at IH
+        rw [IH]
+        · exact nodupKeys.tail
+        · simp [Membership.mem,AList.keys] at *
+          intros mem
+          apply NotIn
+          apply List.Mem.tail
+          apply mem
+end AList
+
+namespace Atom
+  @[aesop safe [constructors, cases]]
+  inductive HasName {α : VarCat i} : Atom α → {β : VarCat i} → Atom β → Prop where
+    | hasName : HasName x x
+
+  @[simp]
+  lemma HasName.to_eq {α : VarCat i} {x y : Atom α} :
+    x.HasName y ↔ x = y
+  := by aesop
+
+  @[simp]
+  lemma HasName.comm {α β : VarCat i} {x : Atom α} {y : Atom β} :
+    x.HasName y ↔ y.HasName x
+  := by aesop
+
+  @[aesop unsafe 20%]
+  instance decidableHasName {α β : VarCat i} (x : Atom α) (y : Atom β) : Decidable (x.HasName y) := by
+    cases decEq α β
+    · case isFalse Neq.cat =>
+      apply isFalse
+      intros hasName
+      cases hasName
+      exact Neq.cat rfl
+    · case isTrue Eq.cat =>
+      cases Eq.cat
+      cases decEq x y
+      · case isFalse Neq.name =>
+        apply isFalse
+        intros hasName
+        cases hasName
+        exact Neq.name rfl
+      · case isTrue Eq.name =>
+        apply isTrue
+        cases Eq.name
+        constructor
+end Atom
+
+@[aesop [unsafe constructors 80%, unsafe cases 10%]]
+inductive Binding : VarCat i → Type :=
+  | val : Typ i → Binding (var i)
+  | sub : Typ i → Binding (tvar i)
+  | typ [HasFeature i type_bindings] : Typ i → Binding (tvar i)
+  deriving DecidableEq
 
 set_option genInjectivity false
+@[aesop safe [constructors, cases]]
 structure Binder (i : CC) where
   cat : VarCat i
   name : Atom cat
   deriving DecidableEq
 
 namespace Binder
-  def freeVariablesVar (b : Binder i) : Finset (Atom (var i)) :=
-    match b with
-    | ⟨var _, x⟩ => {x}
-    | ⟨tvar _, _⟩ => ∅
+  @[simp]
+  def dom {α : VarCat i} (b : Binder i) : Finset (Atom α) :=
+    if h : b.cat = α then
+      {h ▸ b.name}
+    else
+      ∅
 
-  def freeVariablesTVar (b : Binder i) : Finset (Atom (tvar i)) :=
-    match b with
-    | ⟨var _, _⟩ => ∅
-    | ⟨tvar _, X⟩ => {X}
+  @[simp]
+  lemma eq_rect :
+    ({ cat := α, name := x } : Binder i) = { cat := β, name := y } ↔ if h : α = β then h ▸ x = y else False
+  := by
+    apply Iff.intro
+    · case mp =>
+      intros Eq
+      injection Eq with Eq.cat Eq.name
+      aesop
+    · case mpr =>
+      aesop
 
-  instance : FreeVariables (Binder i) (var i) where
-    fv := freeVariablesVar
+  @[aesop safe [constructors, cases]]
+  inductive HasName : Binder i → {α : VarCat i} → Atom α → Prop where
+    | hasName : HasName ⟨α, x⟩ x
 
-  instance : FreeVariables (Binder i) (tvar i) where
-    fv := freeVariablesTVar
+  @[simp]
+  lemma HasName.to_eq {v : Binder i} {x : Atom v.cat} :
+    v.HasName x ↔ v.name = x
+  := by aesop
+
+  @[aesop unsafe 20%]
+  lemma HasName.in_dom {α : VarCat i} {v : Binder i} {x : Atom α} :
+    v.HasName x ↔ x ∈ Binder.dom v
+  := by
+    simp only [Binder.dom]
+    cases α <;> cases v <;> aesop
+
+  @[simp]
+  lemma HasName.name {v : Binder i} {x : Atom α} :
+    v.HasName x ↔ v.name.HasName x
+  := by aesop
+
+  @[simp]
+  lemma HasName.comm {α : VarCat i} {v : Binder i} {x : Atom α} :
+    v.HasName x ↔ x.HasName v.name
+  := by aesop
+
+  @[aesop safe]
+  instance decidableHasName (v : Binder i) {α : VarCat i} (x : Atom α) : Decidable (v.HasName x) := by
+    cases Atom.decidableHasName v.name x
+    · case isFalse hasn'tName =>
+      apply isFalse
+      intros hasName
+      cases hasName
+      apply hasn'tName
+      constructor
+    · case isTrue hasName =>
+      apply isTrue
+      cases hasName
+      constructor
 end Binder
 
+@[aesop unsafe [constructors 10%, cases 40%]]
 inductive Assoc (i : CC) : Type where
-  | var : Atom (var i) -> Typ i -> Assoc i
-  | sub : Atom (tvar i) -> Typ i -> Assoc i
-  | typ [HasFeature i type_bindings] : Atom (tvar i) -> Typ i -> Assoc i
+  | val : Atom (var i) → Typ i → Assoc i
+  | sub : Atom (tvar i) → Typ i → Assoc i
+  | typ [HasFeature i type_bindings] : Atom (tvar i) → Typ i → Assoc i
+  deriving DecidableEq
 
 namespace Assoc
-  infix:65 " ⦂ " => Assoc.var
-  infix:65 " <: " => Assoc.sub
-  infix:65 " ≔ " => Assoc.typ
+  infix:80 " ⦂ " => Assoc.val
+  infix:80 " <: " => Assoc.sub
+  infix:80 " ≔ " => Assoc.typ
 
+  @[aesop norm]
+  def type : Assoc i → Typ i
+    | .val _ T => T
+    | .sub _ S => S
+    | @Assoc.typ _ _ _ T => T
+
+  @[aesop norm]
+  def binder : Assoc i → Binder i
+    | .val x _ => ⟨.var _, x⟩
+    | .sub X _ => ⟨.tvar _, X⟩
+    | @Assoc.typ _ _ X _ => ⟨.tvar _, X⟩
+
+  @[aesop norm]
+  def name (a : Assoc i) : Atom a.binder.cat :=
+    a.binder.name
+
+  @[simp] lemma name_val : (x ⦂  T).name = x := rfl
+  @[simp] lemma name_sub : (X <: S).name = X := rfl
+  @[simp] lemma name_typ : (X ≔  T).name = X := rfl
+
+  @[aesop norm]
+  def cat (a : Assoc i) : VarCat i :=
+    a.binder.cat
+
+  @[simp] lemma cat_val {x : Atom (var i)}  : (x ⦂  T).cat = var i := rfl
+  @[simp] lemma cat_sub {X : Atom (tvar i)} : (X <: S).cat = tvar i := rfl
+  @[simp] lemma cat_typ {X : Atom (tvar i)} : (X ≔  T).cat = tvar i := rfl
+
+  @[aesop norm]
+  def dom {α : VarCat i} (a : Assoc i) : Finset (Atom α) :=
+    a.binder.dom
+
+  @[simp] lemma dom_var_val  {x : Atom (var i)}  : (x ⦂  T).dom = {x} := rfl
+  @[simp] lemma dom_tvar_sub {X : Atom (tvar i)} : (X <: S).dom = {X} := rfl
+  @[simp] lemma dom_tvar_typ {X : Atom (tvar i)} : (X ≔  T).dom = {X} := rfl
+
+  @[simp] lemma dom_tvar_val {x : Atom (var i)}  : (x ⦂  T).dom (α := tvar i) = ∅ := rfl
+  @[simp] lemma dom_var_sub  {X : Atom (tvar i)} : (X <: S).dom (α := var i) = ∅ := rfl
+  @[simp] lemma dom_var_typ  {X : Atom (tvar i)} : (X ≔  T).dom (α := var i) = ∅ := rfl
+
+  @[simp]
+  lemma val_inj : (x ⦂  T) = (x' ⦂  T') ↔ x = x' ∧ T = T'
+  := by
+    apply Iff.intro
+    · case mp =>
+      intros eq
+      injection eq with eq.name eq.type
+      apply And.intro eq.name eq.type
+    · case mpr => aesop
+
+  @[simp]
+  lemma sub_inj : (X <: S) = (X' <: S') ↔ X = X' ∧ S = S'
+  := by
+    apply Iff.intro
+    · case mp =>
+      intros eq
+      injection eq with eq.name eq.type
+      apply And.intro eq.name eq.type
+    · case mpr => aesop
+
+  @[simp]
+  lemma typ_inj : (X ≔  T) = (X' ≔  T') ↔ X = X' ∧ T = T'
+  := by
+    apply Iff.intro
+    · case mp =>
+      intros eq
+      injection eq with eq.name eq.type
+      apply And.intro eq.name eq.type
+    · case mpr => aesop
+
+  @[simp]
   def fromSigma (p : (v : Binder i) × Binding v.cat) : Assoc i :=
     match p with
-    | ⟨⟨.var _, x⟩, .val T⟩ => .var x T
-    | ⟨⟨.tvar _, X⟩, .sub S⟩ => .sub X S
-    | ⟨⟨.tvar _, X⟩, @Binding.typ _ _ T⟩ => .typ X T
+    | ⟨⟨_, x⟩, .val T⟩ => .val x T
+    | ⟨⟨_, X⟩, .sub S⟩ => .sub X S
+    | ⟨⟨_, X⟩, @Binding.typ _ _ T⟩ => .typ X T
 
+  @[simp]
+  def toSigma : Assoc i → (v : Binder i) × Binding v.cat
+    | .val x T => ⟨⟨_, x⟩, .val T⟩
+    | .sub X S => ⟨⟨_, X⟩, .sub S⟩
+    | @Assoc.typ _ _ X T => ⟨⟨_, X⟩, .typ T⟩
+
+  @[simp]
+  def fromSigma_toSigma {a : Assoc i} :
+    fromSigma (toSigma a) = a
+  := by cases a <;> simp
+
+  @[simp]
+  def toSigma_fromSigma {B : (v : Binder i) × Binding v.cat} :
+    toSigma (fromSigma B) = B
+  := by
+    obtain ⟨⟨α, x⟩, b⟩ := B
+    simp at b
+    cases b <;> simp
+
+  @[simp]
+  def isoSigma :
+    Assoc i ≃ ((v : Binder i) × Binding v.cat)
+  := by
+    apply Equiv.mk toSigma fromSigma
+    · case left_inv =>
+      apply fromSigma_toSigma
+    · case right_inv =>
+      apply toSigma_fromSigma
+
+  @[simp]
+  lemma binder_fromSigma_eq_fst :
+    binder (fromSigma B) = B.fst
+  := by
+    obtain ⟨v, b⟩ := B
+    cases v; cases b <;> simp [fromSigma,binder]
+
+  @[simp]
+  lemma dom_fromSigma_def {α β : VarCat i} {x : Atom β} {b : Binding β} :
+    dom (fromSigma ⟨⟨β, x⟩, b⟩) (α := α) =
+      if h : α = β then
+        {h ▸ x}
+      else ∅
+  := by
+    simp only [dom,Binder.dom]
+    rw [binder_fromSigma_eq_fst]
+    split
+    · case inl Eq.cat =>
+      cases Eq.cat
+      simp
+    · case inr Neq.cat =>
+      replace Neq.cat : α ≠ β := Neq.cat ∘ Eq.symm
+      simp [Neq.cat]
+
+  @[simp]
+  lemma dom_fromSigma {α : VarCat i} {x : Atom α} {b : Binding α} :
+    dom (fromSigma ⟨⟨α, x⟩, b⟩) (α := α) = {x}
+  := by
+    simp only [dom,Binder.dom]
+    rw [binder_fromSigma_eq_fst]
+    split
+    · case inl Eq.cat =>
+      cases Eq.cat
+      simp
+    · case inr Neq.cat =>
+      simp at Neq.cat
+
+  @[simp]
   lemma fromSigma_inj :
-      Assoc.fromSigma p1 = Assoc.fromSigma p2 →
-      p1 = p2
-    := by
-      intros eq
-      cases p1; rename_i x b1; cases p2; rename_i y b2
-      cases x; rename_i c x; cases y; rename_i d y
-      cases b1 <;> cases b2 <;> rename_i T U <;> cases eq <;> rfl
+    fromSigma p1 = fromSigma p2 →
+    p1 = p2
+  := by
+    intros eq
+    cases p1; rename_i x b1; cases p2; rename_i y b2
+    cases x; rename_i c x; cases y; rename_i d y
+    cases b1 <;> cases b2 <;> rename_i T U <;> cases eq <;> rfl
 
-  def freeVariablesVar (a : Assoc i) : Finset (Atom (.var i)) :=
-    match a with
-    | .var x _ => {x}
-    | .sub _ _ => ∅
-    | @Assoc.typ _ _ _ _ => ∅
+  @[aesop [safe constructors, unsafe cases 70%]]
+  inductive HasName : Assoc i → {α : VarCat i} → Atom α → Prop where
+    | val x T : HasName (x ⦂  T) x
+    | sub X S : HasName (X <: S) X
+    | typ X T : HasName (X ≔  T) X
 
-  def freeVariablesTVar (a : Assoc i) : Finset (Atom (.tvar i)) :=
-    match a with
-    | .var _ _ => ∅
-    | .sub X _ => {X}
-    | @Assoc.typ _ _ X _ => {X}
+  @[simp]
+  lemma HasName.to_eq {a : Assoc i} {x : Atom a.cat} :
+    a.HasName x ↔ a.name = x
+  := by aesop
 
-  instance : FreeVariables (Assoc i) (.var i) where
-    fv := freeVariablesVar
+  @[aesop unsafe 20%]
+  lemma HasName.in_dom {α : VarCat i} {a : Assoc i} {x : Atom α} :
+    a.HasName x ↔ x ∈ Assoc.dom a
+  := by
+    simp only [Assoc.dom,Assoc.binder]
+    cases α <;> cases a <;> aesop
 
-  instance : FreeVariables (Assoc i) (.tvar i) where
-    fv := freeVariablesTVar
+  lemma HasName.binder {a : Assoc i} {x : Atom α} :
+    a.HasName x ↔ a.binder.HasName x
+  := by aesop
+
+  lemma HasName.name {a : Assoc i} {x : Atom α} :
+    a.HasName x ↔ a.name.HasName x
+  := by aesop
+
+  @[simp]
+  lemma HasName.comm {α : VarCat i} {a : Assoc i} {x : Atom α} :
+    a.HasName x ↔ x.HasName a.name
+  := by aesop
+
+  @[aesop unsafe 20%]
+  instance decidableHasName (a : Assoc i) {α : VarCat i} (x : Atom α) : Decidable (a.HasName x)
+  := by
+    cases Binder.decidableHasName a.binder x
+    · case isFalse hasn'tName =>
+      apply isFalse
+      intros hasName
+      cases hasName
+        <;> simp [binder] at hasn'tName
+    · case isTrue hasName =>
+      apply isTrue
+      cases a
+        <;> simp [binder] at hasName
+        <;> cases hasName
+        <;> constructor
 end Assoc
 
 abbrev Env (i : CC) := AList (fun (v : Binder i) => Binding v.cat)
@@ -86,55 +380,651 @@ abbrev Env (i : CC) := AList (fun (v : Binder i) => Binding v.cat)
 namespace Env
   def cons (Γ : Env i) (a : Assoc i) : Env i :=
     match a with
-    | .var x T => AList.insert ⟨var i, x⟩ (Binding.val T) Γ
-    | .sub X S => AList.insert ⟨tvar i, X⟩ (Binding.sub S) Γ
-    | @Assoc.typ _ _ X T => AList.insert ⟨tvar i, X⟩ (Binding.typ T) Γ
+    | .val x T => AList.insert ⟨_, x⟩ (Binding.val T) Γ
+    | .sub X S => AList.insert ⟨_, X⟩ (Binding.sub S) Γ
+    | @Assoc.typ _ _ X T => AList.insert ⟨_, X⟩ (Binding.typ T) Γ
 
-  infixl:60 " ▷ " => Env.cons
+  infixl:70 " ▷ " => Env.cons
 
-  def assocs (Γ : Env i) : Finset (Assoc i) :=
-    Finset.mk
-      (Multiset.ofList (Γ.entries.map Assoc.fromSigma))
-      (List.Nodup.map_on fromSigma_inj_Γ nodupKeys_nodupEntries)
-  where
-      nodupKeys_nodupEntries : Γ.entries.Nodup := by
-        cases Γ; rename_i entries nodupKeys
-        simp [AList.keys] at nodupKeys
-        induction entries <;> simp
-        case cons head tail IH =>
-          cases head; rename_i x b; simp at nodupKeys
-          cases nodupKeys; rename_i xNotInTail nodupTail
-          apply And.intro
-          · intros H
-            apply xNotInTail
-            simp [List.keys] at *
-            exists b
-          · apply IH
-            apply nodupTail
+  def fold (f : α → Assoc i → α) (init : α) (Γ : Env i) : α :=
+    List.foldr (fun s acc => f acc (Assoc.fromSigma s)) init Γ.entries
 
-      fromSigma_inj_Γ :
-        ∀ x ∈ Γ.entries, ∀ y ∈ Γ.entries,
-        Assoc.fromSigma x = Assoc.fromSigma y
-        → x = y
-      := by
-        intros
-        apply Assoc.fromSigma_inj
-        assumption
+  def assocs (Γ : Env i) : List (Assoc i) :=
+    Γ.entries.map Assoc.fromSigma
 
   def binders (Γ : Env i) : Finset (Binder i) :=
     Finset.mk (Multiset.ofList Γ.keys) Γ.nodupKeys
 
-  def dom (Γ : Env i) (α : VarCat i) [FreeVariables (Binder i) α] : Finset (Atom α) :=
-    Finset.fold (fun s t => s ∪ t) ∅ FreeVariables.fv Γ.binders
+  def bindersList (Γ : Env i) : List (Binder i) :=
+    Γ.keys
+
+  def dom (Γ : Env i) {α : VarCat i} : Finset (Atom α) :=
+    fold (· ∪ Assoc.dom ·) ∅ Γ
+
+  def erase {α : VarCat i} (Γ : Env i) (x : Atom α) : Env i :=
+    AList.erase ⟨α, x⟩ Γ
+
+  @[simp]
+  def cons_eq_iff :
+    Γ ▷ a = Δ ▷ b ↔ erase Γ a.name = erase Δ b.name ∧ a = b
+  := by
+    apply Iff.intro
+    · intros Eq
+      simp [erase,AList.erase]
+      simp [cons] at Eq
+      cases a <;> rename_i x T <;> cases b <;> rename_i x' T'
+        <;> simp [AList.insert] at Eq
+        <;> obtain ⟨⟨Eq.x, Eq.T⟩, Eq.tl⟩ := Eq
+        <;> simp [Assoc.binder]
+      all_goals apply And.intro <;> aesop
+    · intros Eqs
+      obtain ⟨Eq.ctx, Eq.asc⟩ := Eqs
+      simp [cons]
+      cases a <;> rename_i x T <;> cases b <;> rename_i x' T'
+        <;> cases Eq.asc
+        <;> simp [AList.insert]
+        <;> simp [erase,AList.erase] at Eq.ctx
+        <;> exact Eq.ctx
+
+  @[simp]
+  def erase_cons_swap {α : VarCat i} {a : Assoc i} {x : Atom α} :
+    ¬a.HasName x →
+    erase (Γ ▷ a) x = erase Γ x ▷ a
+  := by
+    intros Neq
+    apply AList.ext
+    simp only [cons]
+    cases α <;> cases a <;> rename_i y T
+      <;> simp only [Assoc.type.match_1]
+      <;> rw [AList.insert_entries]
+      <;> simp only [erase,AList.erase]
+      <;> simp only [AList.insert,List.kinsert]
+      <;> rw [List.kerase_cons_ne (by aesop)]
+      <;> rw [List.kerase_kerase]
+
+  @[simp]
+  lemma erase_nil :
+    erase ∅ x = ∅
+  := by rfl
+
+  @[simp]
+  lemma fold_nil :
+    fold f z ∅ = z
+  := by rfl
+
+  @[simp]
+  lemma fold_cons :
+    fold f z (Γ ▷ a) = f (fold f z (erase Γ a.name)) a
+  := by
+    cases a <;> simp [fold,cons,erase,AList.erase,Assoc.binder]
+
+  @[simp]
+  lemma erase_cons_eq {i : CC} {Γ : Env i} {a : Assoc i} :
+    erase (Γ ▷ a) a.name = erase Γ a.name
+  := by
+    cases a <;> rename_i x T <;> simp [erase,cons,AList.erase,Assoc.binder]
+
+  @[simp]
+  lemma erase_cons {i : CC} {α : VarCat i} {Γ : Env i} (a : Assoc i) {x : Atom α} :
+    erase (Γ ▷ a) x =
+      if a.HasName x then
+        erase Γ x
+      else
+        erase Γ x ▷ a
+  := by
+    split
+    · case inl hasName =>
+      cases hasName <;> simp [erase,cons,AList.erase]
+    · case inr hasn'tName =>
+      cases a
+        <;> simp only [erase,cons]
+        <;> rw [AList.insert_erase]
+        <;> simp
+        <;> split
+        <;> first | simp
+                  | rename_i Eq.cat;
+                    cases Eq.cat;
+                    simp;
+                    intros Eq.name;
+                    cases Eq.name;
+                    apply hasn'tName;
+                    constructor
+
+  lemma binder_mem_iff_name_mem_dom {α : VarCat i} {x : Atom α} :
+    ⟨α, x⟩ ∈ Γ ↔ x ∈ dom Γ
+  := by
+    induction Γ using AList.insertRec
+    · case H0 => simp [dom,assocs]
+    · case IH w b Γ w.NotIn IH =>
+      apply Iff.intro
+      · case mp =>
+        intros v.In
+        cases v.In <;> simp only [dom,fold,assocs,List.map,List.foldr,Finset.mem_union]
+        · case head =>
+          apply Or.inr
+          rw [Assoc.dom_fromSigma]
+          simp
+        · case tail v.In =>
+          cases (decEq ⟨α, x⟩ w)
+          · case isFalse neq =>
+            apply Or.inl
+            rw [List.kerase_of_not_mem_keys (by aesop)] at *
+            apply IH.mp v.In
+          · case isTrue eq =>
+            apply Or.inr
+            obtain ⟨β, y⟩ := w
+            injection eq with eq.cat eq.name
+            simp at b
+            rw [eq.cat,eq.name,Assoc.dom_fromSigma]
+            simp
+      · case mpr =>
+        intros v.In
+        simp only [dom,assocs,fold,List.foldr,Finset.mem_union] at v.In
+        simp
+        cases v.In
+        · case inl v.In =>
+          cases (decEq ⟨α, x⟩ w)
+          · case isFalse neq =>
+            apply Or.inr
+            rw [List.kerase_of_not_mem_keys (by aesop)] at v.In
+            apply IH.mpr
+            simp [dom,Finset.fold,AList.keys,List.keys]
+            apply v.In
+          · case isTrue eq =>
+            rw [eq]
+            apply Or.inl rfl
+        · case inr v.In =>
+          apply Or.inl
+          obtain ⟨β, y⟩ := w
+          simp at b
+          simp only [Assoc.dom] at v.In
+          rw [Assoc.binder_fromSigma_eq_fst] at v.In
+          simp [Binder.dom] at v.In
+          simp
+          split
+          · case inl Eq.cat =>
+            simp [Eq.cat] at v.In
+            cases Eq.cat
+            exact v.In
+          · case inr Neq.cat =>
+            replace Neq.cat : β ≠ α := Neq.cat ∘ Eq.symm
+            simp [Neq.cat] at v.In
+
+  @[elab_as_elim]
+  lemma rec_erase {motive : Env i → Sort}
+    (nil : motive ∅)
+    (cons : ∀ (Γ : Env i) (a : Assoc i),
+      motive (erase Γ a.name) →
+      motive (Γ ▷ a))
+    : ∀ Γ, motive Γ
+  := by
+    intros Γ
+    induction Γ using AList.insertRec
+    · case H0 => exact nil
+    · case IH v b Γ v.NotIn IH =>
+      specialize cons Γ (Assoc.fromSigma ⟨v, b⟩)
+      simp [erase,_root_.Env.cons] at cons
+      obtain ⟨α, x⟩ := v
+      cases b <;> simp [Assoc.binder] at cons
+        <;> apply cons
+        <;> rw [AList.erase_of_not_mem v.NotIn]
+        <;> exact IH
+
+  @[elab_as_elim]
+  lemma rec_assoc {motive : Env i → Sort}
+    (nil : motive ∅)
+    (cons : ∀ (Γ : Env i) (a : Assoc i),
+      a.name ∉ dom Γ →
+      motive Γ →
+      motive (Γ ▷ a))
+    : ∀ Γ, motive Γ
+  := by
+    intros Γ
+    induction Γ using AList.insertRec
+    · case H0 =>
+      exact nil
+    · case IH v b Γ v.NotIn IH =>
+      specialize cons Γ (Assoc.fromSigma ⟨v, b⟩)
+      cases v; cases b
+        <;> rw [Assoc.binder_fromSigma_eq_fst] at cons
+        <;> simp only [_root_.Env.cons,Assoc.fromSigma,Assoc.binder] at cons
+        <;> apply cons (binder_mem_iff_name_mem_dom.not.mp v.NotIn) IH
+
+  @[elab_as_elim,eliminator]
+  lemma rec_bindings {motive : Env i → Sort}
+    (nil : motive ∅)
+    (val : ∀ (x : Atom (.var i)) (T : Typ i) (Γ : Env i),
+      x ∉ dom Γ →
+      motive Γ →
+      motive (Γ ▷ x ⦂ T))
+    (sub : ∀ (X : Atom (.tvar i)) (T : Typ i) (Γ : Env i),
+      X ∉ dom Γ →
+      motive Γ →
+      motive (Γ ▷ X <: T))
+    (typ : ∀ (X : Atom (.tvar i)) (T : Typ i) (Γ : Env i),
+      X ∉ dom Γ →
+      motive Γ →
+      motive (Γ ▷ X ≔ T))
+    : ∀ Γ, motive Γ
+  := by
+    intros Γ
+    induction Γ using rec_assoc
+    · case nil => exact nil
+    · case cons Γ a a.NotIn IH =>
+      cases a
+      · case val => apply val <;> aesop
+      · case sub => apply sub <;> aesop
+      · case typ => apply typ <;> aesop
+
+  lemma dom_keys {α : VarCat i} {x : Atom α} {Γ : Env i} :
+    x ∈ dom Γ ↔ ⟨α, x⟩ ∈ Γ.keys
+  := by
+    simp only [dom,fold,AList.keys]
+    induction Γ.entries generalizing α
+    · case nil => simp
+    · case cons s Γ.entries IH =>
+      simp only [List.foldr,List.keys,List.map]
+      simp only [Finset.mem_union,List.mem_cons]
+      apply Iff.intro
+      · case mp =>
+        intros x.In
+        cases x.In
+        · case inl x.In =>
+          apply Or.inr
+          apply IH.mp x.In
+        · case inr x.In =>
+          apply Or.inl
+          obtain ⟨⟨β, y⟩, b⟩ := s
+          simp only [Assoc.dom_fromSigma_def] at x.In
+          simp
+          split
+          · case inl Eq.cat =>
+            simp [Eq.cat] at x.In
+            cases Eq.cat
+            exact x.In
+          · case inr Neq.cat =>
+            simp [Neq.cat] at x.In
+      · case mpr =>
+        intros x.In
+        cases x.In
+        · case inl x.In =>
+          apply Or.inr
+          obtain ⟨⟨β, y⟩, b⟩ := s
+          simp only [Assoc.dom_fromSigma_def]
+          split
+          · case inl Eq.cat =>
+            simp [Eq.cat] at x.In
+            cases Eq.cat
+            simp
+            exact x.In
+          · case inr Neq.cat =>
+            simp [Neq.cat] at x.In
+        · case inr x.In =>
+          apply Or.inl
+          apply IH.mpr x.In
+
+  @[simp]
+  lemma dom_nil {α : VarCat i} : dom (α := α) ∅ = ∅
+  := by simp [dom]
+
+  lemma dom_cons_weak {Γ : Env i} {a : Assoc i} :
+    dom (Γ ▷ a) (α := α) = dom (erase Γ a.name) ∪ Assoc.dom a
+  := by simp [dom]
+
+  @[simp]
+  lemma erase_not_in_dom {Γ : Env i} {x : Atom α} :
+    x ∉ dom Γ →
+    erase Γ x = Γ
+  := by
+    intros x.NotIn
+    simp [erase]
+    rw [dom_keys] at x.NotIn
+    apply AList.erase_of_not_mem x.NotIn
+
+  lemma erase_commutative :
+    erase (erase Γ x) y = erase (erase Γ y) x
+  := by
+    simp [erase]
+    apply AList.erase_erase
+
+  @[simp]
+  lemma erase_in {Γ : Env i} {α β : VarCat i} {x : Atom α} {y : Atom β} :
+    x ∈ dom (erase Γ y) ↔ x ∈ dom Γ ∧ ¬x.HasName y
+  := by
+    induction Γ <;> simp
+    all_goals {
+      rename_i z T Γ z.NotIn IH
+      split
+      · case inl hasName =>
+        cases hasName
+        all_goals {
+          simp [dom_cons_weak,Assoc.name,Assoc.binder]
+          rw [erase_not_in_dom z.NotIn] at *
+          aesop
+        }
+      · case inr hasn'tName =>
+        simp [dom_cons_weak,Assoc.name,Assoc.dom,Assoc.binder]
+        rw [erase_commutative]
+        rw [erase_not_in_dom z.NotIn]
+        cases α <;> first | simp at hasn'tName
+                          | aesop
+    }
+
+  lemma erase_notin {α β : VarCat i} {x : Atom α} {y : Atom β} :
+    x ∉ dom Γ →
+    x ∉ dom (erase Γ y)
+  := by
+    intros x.NotIn
+    induction Γ using rec_assoc generalizing α β <;> simp
+    case cons Γ a a.NotIn IH =>
+    split
+    · case inl hasName =>
+      cases hasName
+      simp only [dom_cons_weak] at x.NotIn
+      aesop
+    · case inr hasn'tName =>
+      rw [dom_cons_weak] at *
+      rw [erase_commutative]
+      rw [erase_not_in_dom a.NotIn] at *
+      simp at *
+      intros x.In
+      rcases x.In with ⟨x.In,x.hasn'tName⟩ | ⟨x.In⟩ <;> apply x.NotIn
+      · exact Or.inl x.In
+      · exact Or.inr x.In
+
+  lemma dom_erase_subset {Γ : Env i} {α β : VarCat i} (x : Atom β) :
+    dom (erase Γ x) (α := α) ⊆ dom Γ
+  := by
+    induction Γ
+    · case nil => simp
+    all_goals {
+      rename_i y T Γ y.NotIn IH
+      simp
+      split
+      · case inl hasName =>
+        cases hasName
+        rw [dom_cons_weak]
+        simp
+        apply Finset.subset_union_left
+      · case inr hasn'tName =>
+        simp only [dom_cons_weak,Assoc.name,Assoc.binder]
+        rw [erase_commutative]
+        rw [erase_not_in_dom y.NotIn]
+        apply Finset.union_subset_union_left IH
+    }
+
+  @[simp]
+  lemma dom_erase {Γ : Env i} {α β : VarCat i} {x : Atom β} :
+    dom (erase Γ x) (α := α) =
+      if h : α = β then
+        dom Γ \ {h ▸ x}
+      else
+        dom Γ
+  := by
+    induction Γ using rec_assoc generalizing x
+    · case nil => simp
+    · case cons Γ a a.NotIn IH =>
+      rw [dom_cons_weak]
+      cases a <;> rename_i y T <;> simp at a.NotIn <;> simp
+      all_goals {
+        split
+        · case inl hasName =>
+          cases hasName
+          rw [erase_not_in_dom a.NotIn]
+          simp [Assoc.binder] at *
+          split
+          · case inl Eq.cat =>
+            cases Eq.cat
+            simp at *
+            aesop
+          · case inr Neq.cat =>
+            cases α <;> simp; exfalso; exact Neq.cat rfl
+        · case inr hasn'tName =>
+          rw [
+            dom_cons_weak,
+            erase_commutative,
+            erase_not_in_dom a.NotIn
+          ]
+          aesop
+      }
+
+  @[simp]
+  lemma dom_cons {Γ : Env i} {a : Assoc i} :
+    dom (Γ ▷ a) (α := α) = dom Γ ∪ Assoc.dom a
+  := by
+    rw [dom_cons_weak]
+    simp [dom_erase]
+    cases α <;> cases a <;> simp [Assoc.binder]
+
+  @[simp]
+  lemma dom_erase_different_cat {Γ : Env i} :
+    α ≠ β →
+    dom (α := β) (erase (α := α) Γ x) = dom Γ
+  := by induction Γ <;> simp [erase_cons,Assoc.binder] <;> aesop
 
   instance instEmptyCollection : EmptyCollection (Env i) where
     emptyCollection := ∅
 
-  instance instAssocMembership : Membership (Assoc i) (Env i) :=
+  instance instMembership : Membership (Assoc i) (Env i) :=
     ⟨fun a Γ => a ∈ Γ.assocs⟩
+
+  @[simp]
+  lemma not_mem_nil (a : Assoc i) :
+    a ∉ (∅ : Env i)
+  := by
+    simp [EmptyCollection.emptyCollection,Membership.mem,assocs]
+    intros a.In
+    cases a.In
+
+  @[simp]
+  lemma assocs_nil :
+    assocs (∅ : Env i) = ∅
+  := by simp [assocs]
+
+  @[simp]
+  lemma assocs_cons :
+    assocs (Γ ▷ a) = a :: assocs (erase Γ a.name)
+  := by aesop
+
+  @[simp]
+  lemma assocs_erase {Γ : Env i} {x : Atom α} :
+    assocs (erase Γ x) = List.eraseP
+      (fun (a : Assoc i) => decide (a.HasName x))
+      (assocs Γ)
+  := by
+    simp only [assocs]
+    rw [List.eraseP_map]
+    simp only [erase,AList.erase,List.kerase]
+    congr
+    ext a
+    simp
+    obtain ⟨v, b⟩ := a
+    cases v; cases b <;> simp
+    all_goals {
+      rename_i T x
+      split
+      · rename_i Eq.cat
+        cases Eq.cat
+        simp
+      · rename_i Neq.cat
+        replace Neq.cat : _ ≠ α := Neq.cat ∘ Eq.symm
+        simp [Neq.cat]
+        intros hasName
+        cases hasName
+        exact Neq.cat rfl
+    }
+
+  @[simp]
+  lemma mem_cons (a b : Assoc i) :
+    a ∈ Γ ▷ b ↔ a ∈ erase Γ b.name ∨ a = b
+  := by
+    simp only [instMembership]
+    rw [assocs_cons]
+    simp only [assocs,erase,assocs_erase,AList.erase,List.kerase]
+    aesop
+
+  def concat (Γ : Env i) (Δ : Env i) : Env i :=
+    Δ ∪ Γ
+
+  instance instAppend : Append (Env i) where
+    append := concat
+
+  @[simp]
+  lemma nil_concat {Γ : Env i} :
+    ∅ ++ Γ = Γ
+  := by simp [HAppend.hAppend,Append.append,concat]
+
+  @[simp]
+  lemma concat_nil {Γ : Env i} :
+    Γ ++ ∅ = Γ
+  := by rfl
+
+  @[simp]
+  lemma concat_singleton {Γ : Env i} :
+    Γ ++ ∅ ▷ a = Γ ▷ a
+  := by cases a <;> rfl
+
+  @[simp]
+  lemma concat_cons {Γ : Env i} :
+    Γ ++ Δ ▷ a = (Γ ++ Δ) ▷ a
+  := by cases a <;> simp [HAppend.hAppend,Append.append,concat,cons,Union.union,AList.union,AList.insert]
+
+  @[simp]
+  lemma erase_concat {Γ Δ : Env i} :
+    erase (Γ ++ Δ) x = erase Γ x ++ erase Δ x
+  := by
+    simp [erase,HAppend.hAppend,Append.append,concat]
+    rw [AList.union_erase]
+
+  @[simp]
+  lemma mem_erase_iff {Γ : Env i} {x : Atom α} {a : Assoc i} :
+    a ∈ erase Γ x ↔ a ∈ Γ ∧ ¬a.HasName x
+  := by
+    induction Γ using rec_assoc <;> simp
+    case cons Γ b b.NotIn IH =>
+    split
+    · case inl hasName =>
+      cases hasName
+      aesop
+    · case inr hasn'tName =>
+      rw [mem_cons]
+      rw [erase_commutative]
+      simp [erase_not_in_dom b.NotIn]
+      aesop
+
+  @[simp]
+  lemma mem_in :
+    a ∈ Γ →
+    a.name ∈ dom Γ
+  := by induction Γ <;> aesop
+
+  @[simp]
+  lemma mem_concat_iff {Γ Δ : Env i} :
+    a ∈ Γ ++ Δ ↔ (a ∈ Γ ∧ a.name ∉ dom Δ) ∨ a ∈ Δ
+  := by
+    induction Δ using rec_assoc generalizing Γ
+    · case nil => aesop
+    · case cons Δ b b.NotIn IH =>
+      apply Iff.intro
+      · case mp =>
+        simp
+        rw [erase_not_in_dom b.NotIn]
+        intros a.In
+        cases a.In
+        · case inl a.In =>
+          rcases IH.mp a.In with ⟨a.InΓ,a.NotInΔ⟩ | ⟨a.InΔ⟩
+          · cases decEq a b
+            · case isFalse Neq =>
+              apply Or.inl (And.intro _ _)
+              · obtain ⟨a.InΓ, _⟩ := mem_erase_iff.mp a.InΓ
+                apply a.InΓ
+              · intros a.InΔb
+                cases a.InΔb
+                · case inl a.InΔ =>
+                  exact a.NotInΔ a.InΔ
+                · case inr a.EqB =>
+                  cases a <;> cases b <;> rename_i x T y U <;> simp [Assoc.name,Assoc.dom,Assoc.binder] at a.EqB
+                  all_goals {
+                    cases a.EqB
+                    simp at *
+                  }
+            · case isTrue a.Eq =>
+              exact Or.inr (Or.inr a.Eq)
+          · apply Or.inr (Or.inl (And.intro a.InΔ _))
+            cases a <;> cases b <;> rename_i x T y U
+              <;> simp [Assoc.name,Assoc.dom,Assoc.binder] at *
+              <;> intros Eq
+              <;> cases Eq
+              <;> apply b.NotIn
+              <;> exact mem_in a.InΔ
+        · case inr a.Eq =>
+          exact Or.inr (Or.inr a.Eq)
+      · case mpr =>
+        simp
+        rw [erase_not_in_dom b.NotIn]
+        intros a.In
+        rcases a.In with ⟨a.InΓ, a.NotInΔ⟩ | ⟨⟨a.InΓ, a.NotInΔ⟩ | a.Eq⟩
+        · cases decEq a b
+          · case isFalse Neq =>
+            apply Or.inl
+            apply IH.mpr
+            apply Or.inl
+            apply And.intro
+            · apply mem_erase_iff.mpr
+              apply And.intro a.InΓ
+              rw [Assoc.HasName.in_dom]
+              intros a.NotB
+              apply a.NotInΔ
+              cases a <;> cases b <;> rename_i x T y U
+                <;> simp [Assoc.name,Assoc.binder] at *
+                <;> aesop
+            · exact a.NotInΔ ∘ Or.inl
+          · case isTrue Eq =>
+            apply Or.inr Eq
+        · cases a <;> cases b <;> rename_i x T y U
+            <;> simp [Assoc.binder] at *
+            <;> aesop
+        · exact Or.inr a.Eq
+
+  @[simp]
+  lemma mem_cons_head {Γ : Env i} :
+    a ∈ Γ ▷ a
+  := by simp
+
+  @[simp]
+  lemma mem_cons_tail {Γ : Env i} :
+    ¬a.HasName b.name →
+    a ∈ Γ →
+    a ∈ Γ ▷ b
+  := by
+    intros Neq a.In
+    simp [mem_cons] at *
+    apply Or.inl (And.intro a.In Neq)
+
+  @[simp]
+  lemma mem_concat_right {Γ Δ : Env i} :
+    a ∈ Δ →
+    a ∈ Γ ++ Δ
+  := by induction Γ <;> aesop
+
+  @[simp]
+  lemma cons_not_nil {Γ : Env i} :
+    Γ ▷ a ≠ ∅
+  := by cases a <;> simp [cons,AList.insert,instEmptyCollection,AList.instEmptyCollectionAList]
+
+  @[simp]
+  lemma dom_concat {Γ Δ : Env i} :
+    dom (α := α) (Γ ++ Δ) = dom Γ ∪ dom Δ
+  := by
+    induction Δ <;> simp [Assoc.dom,Assoc.binder]
+    all_goals {
+      rename_i IH
+      split <;> simp [IH]
+    }
 end Env
 
 attribute [irreducible] Env
 
-instance : EmptyCollection (Env i) := Env.instEmptyCollection
-instance : Membership (Assoc i) (Env i) := Env.instAssocMembership
+@[simp] instance : EmptyCollection (Env i) := Env.instEmptyCollection
+@[simp] instance : Membership (Assoc i) (Env i) := Env.instMembership
+@[simp] instance : Append (Env i) := Env.instAppend
