CCDeconstructed/Syntax.lean
@@ -1,33 +1,34 @@
 import CCDeconstructed.CC
 import CCDeconstructed.Var
 
+import Mathlib.Data.List.AList
+
 open VarCat Feature
 
-section Syntax
-  variable (i : CC)
+abbrev Cap (i : CC) := Finset (Var (var i))
 
-  abbrev Cap := Finset (Var (var i))
+inductive TypevarKind (i : CC) where
+  | ε : TypevarKind i
+  | sealed [HasFeature i sealed_type_parameters] : TypevarKind i
+  deriving DecidableEq
 
-  inductive TypevarKind where
-    | ε : TypevarKind
-    | sealed [HasFeature i sealed_type_parameters] : TypevarKind
+inductive Typ (i : CC) where
+  | top : Typ i
+  | var : Var (tvar i) → Typ i
+  | arr : Typ i → Typ i → Typ i
+  | all : TypevarKind i → Typ i → Typ i → Typ i
+  | box [HasFeature i .box_type] : Typ i → Typ i
+  | cap : Typ i → Cap i → Typ i
+  deriving DecidableEq
 
-  inductive Typ where
-    | top : Typ
-    | var : Var (tvar i) -> Typ
-    | arr : Typ -> Typ -> Typ
-    | all : TypevarKind i -> Typ -> Typ -> Typ
-    | box [HasFeature i .box_type] : Typ -> Typ
-    | cap : Typ -> Cap i -> Typ
-
-  inductive Exp where
-    | var : Var (var i) -> Exp
-    | abs : Typ i -> Exp -> Exp
-    | app : Var (var i) -> Var (var i) -> Exp
-    | tabs : Typ i -> Exp -> Exp
-    | tapp : Var (var i) -> Typ i -> Exp
-    | let : Exp -> Exp -> Exp
-    | type [HasFeature i type_bindings] : Typ i -> Exp -> Exp
-    | box [HasFeature i explicit_boxing] : Var (var i) -> Exp
-    | unbox [HasFeature i explicit_boxing] : Var (var i) -> Exp
-end Syntax
+inductive Exp (i : CC) where
+  | var : Var (var i) → Exp i
+  | abs : Typ i → Exp i → Exp i
+  | app : Var (var i) → Var (var i) → Exp i
+  | tabs : Typ i → Exp i → Exp i
+  | tapp : Var (var i) → Typ i → Exp i
+  | let_ : Exp i → Exp i → Exp i
+  | type [HasFeature i type_bindings] : Typ i → Exp i → Exp i
+  | box [HasFeature i explicit_boxing] : Var (var i) → Exp i
+  | unbox [HasFeature i explicit_boxing] : Var (var i) → Exp i
+  deriving DecidableEq
