CCDeconstructed/Tactics.lean
@@ -14,7 +14,6 @@ def gatherAtoms {i : Q(CC)} (β : Q(VarCat $i)) : TacticM Q(Finset (Atom $β)) :
       | LocalDecl.ldecl (type := t) .. => t
     match ← trySynthInstanceQ q(FreeVariables $α $β) with
     | .some instFreeVariables => do
-        dbg_trace ("\tok!")
         let x : Q($α) := decl.toExpr
         let fv : Q(Finset (Atom $β)) := q(($instFreeVariables).fv $x)
         return q($acc ∪ $fv)
@@ -31,7 +30,6 @@ def evalPickFresh {i : Q(CC)} {qβ : Q(VarCat $i)} (x : TSyntax `ident) (qL : Q(
 syntax (name := pick_fresh)
   "pick_fresh" ident (":" term)? ("∉" term)? : tactic
 
-/-
 elab_rules (kind := pick_fresh) : tactic
   | `(tactic| pick_fresh $x:ident : $β:term) =>
       withMainContext do
@@ -45,18 +43,80 @@ elab_rules (kind := pick_fresh) : tactic
         let qβ : Q(VarCat $qi) ← mkFreshExprMVar (type? := q(VarCat $qi))
         let qL : Q(Finset (Atom $qβ)) ← runTermElab (elabTerm L (expectedType? := q(Finset (Atom $qβ))))
         evalPickFresh x qL
--/
 
-elab_rules (kind := pick_fresh) : tactic
-  | `(tactic| pick_fresh $x:ident : $β:term) =>
-      withMainContext do
-        let qi : Q(CC) ← mkFreshExprMVar (type? := q(CC))
-        let qβ : Q(VarCat $qi) ← runTermElab (elabTerm β (expectedType? := q(VarCat $qi)))
-        let qL : Q(Finset (Atom $qβ)) ← @gatherAtoms qi qβ
-        evalPickFresh x qL
-  | `(tactic| pick_fresh $x:ident ∉ $L:term) =>
-      withMainContext do
-        let qi : Q(CC) ← mkFreshExprMVar (type? := q(CC))
-        let qβ : Q(VarCat $qi) ← mkFreshExprMVar (type? := q(VarCat $qi))
-        let qL : Q(Finset (Atom $qβ)) ← runTermElab (elabTerm L (expectedType? := q(Finset (Atom $qβ))))
-        evalPickFresh x qL
+structure ScopeInfo where
+  i : Q(CC)
+  α : Q(VarCat $i)
+  x : TSyntax `ident
+  L : Q(Finset (Atom $α))
+  decl : LocalDecl
+
+def findScope : TacticM (Option ScopeInfo) :=
+  withMainContext do
+    (← MonadLCtx.getLCtx).findDeclM? fun decl => do
+      let ty : Q(Prop) :=
+        match decl with
+        | LocalDecl.cdecl (type := t) .. => t
+        | LocalDecl.ldecl (type := t) .. => t
+      -- dbg_trace (← ppExpr ty).pretty
+      match ty with
+      | ~q(∀ x, ¬(@Membership.mem _ _ ⟨_⟩ x $L) → ($p : Atom $α → Prop) x) => do
+          let x : Name := match ty with | .forallE x _ _ _ => x | _ => .anonymous
+          let xIdent : TSyntax `ident := mkIdent x
+          return .some ⟨_, α, xIdent, L, decl⟩
+      | _ => return .none
+
+def specializeAnyScope : TacticM Unit := do
+  match (← findScope) with
+  | .some ⟨qi, qα, x, _, decl⟩ => do
+      let FrIdent := mkIdent (.str (.str .anonymous x.getId.toString) "Fresh")
+      let qL : Q(Finset (Atom $qα)) ← @gatherAtoms qi qα
+      let declIdent := mkIdent decl.userName
+      evalTactic (← `(tactic|
+        cases (Atom.freshFor $(← runTermElab qL.toSyntax));
+        rename_i $x:ident $FrIdent:ident;
+        simp only [Finset.union_empty,Finset.empty_union,Finset.union_assoc,FreeVariables.fv,id] at $FrIdent:ident;
+        specialize $declIdent:ident $x:ident (by aesop);
+      ))
+  | .none => throwTacticEx `specializeAllScopes (← getMainGoal) "couldn't find any goal to specialize"
+
+namespace Playground
+  scoped syntax (name := pick_fresh_any) "pick_fresh_any" : tactic
+  elab_rules (kind := pick_fresh_any) : tactic
+    | `(tactic| pick_fresh_any) =>
+        withMainContext do
+          let _ ← specializeAnyScope
+          return ()
+
+  variable
+    (i : CC)
+    (e1 e2 : Exp i)
+    (z : Atom (.var i)) (Z1 Z2 : Atom (.tvar i))
+    (L1 : Finset (Atom (.var i)))
+    (L2 : Finset (Atom (.tvar i)))
+    (inst : ∀ {α : VarCat i}, Atom α → Exp i → Exp i)
+    (P : Exp i → Prop)
+    (IH1 : ∀ x, x ∉ L1 → P (inst x e1))
+    (IH2 : ∀ Y, Y ∉ L2 → P (inst Y e2))
+
+  example : True := by
+    -- IH1: ∀ x ∉ L1, P (inst x e1)
+    -- IH2: ∀ Y ∉ L2, P (inst Y e2)
+    pick_fresh_any
+    -- IH2: ∀ Y ∉ L2, P (inst Y e2)
+    -- x: Atom (VarCat.var i)
+    -- IH1: P (inst x e1)
+    -- x.Fresh: x ∉ L1
+    pick_fresh_any
+    -- x: Atom (VarCat.var i)
+    -- IH1: P (inst x e1)
+    -- x.Fresh: x ∉ L1
+    -- Y: Atom (VarCat.tvar i)
+    -- IH2: P (inst Y e2)
+    -- Y.Fresh: Y ∉ L2
+    constructor
+
+  attribute [aesop safe tactic] specializeAnyScope
+
+  example : ∃ x ∉ L1, P (inst x e1) := by aesop
+end Playground
