CCDeconstructed/Typing.lean
@@ -1,26 +1,22 @@
 import CCDeconstructed.CC
 import CCDeconstructed.Var
 import CCDeconstructed.Syntax
+import CCDeconstructed.Classes
+import CCDeconstructed.Infrastructure
 import CCDeconstructed.WellFormedness
 
 open Feature VarCat
 
 variable {i : CC}
 
-class Sub (α : Typ) where
-  Rel : Env i -> α -> α -> Prop
-  refl : Reflexive Rel
-  trans : Transitive Rel
-  regular : Rel Γ x y -> WellFormed Γ ∧ WellFormed x ∧ WellFormed y
-
 section Subtyping
   set_option hygiene false
   notation:30 Γ " ⊢ " T " <: " U => Subtyping Γ T U
 
-  inductive Subtyping : Env i -> Typ i -> Typ i -> Prop where
+  inductive Subtyping : Env i → Typ i → Typ i → Prop where
     | reflTvar (X : Atom (tvar i)) :
-        Env.WellFormed Γ ->
-        Atom.WellFormed Γ X ->
+        Env.WellFormed Γ →
+        Atom.WellFormed Γ X →
 
 end Subtyping
 
@@ -29,8 +25,11 @@ notation:30 Γ " ⊢ " T " <: " U => Sub.Rel Γ T U
 set_option hygiene false
 notation:30 C "; " Γ " ⊢ " e " : " T => Typing C Γ e T
 
-inductive Typing : Cap i -> Env i -> Exp i -> Typ i -> Prop :=
+inductive Typing : Cap i → Env i → Exp i → Typ i → Prop :=
   | var (x : Atom (var i)) :
-      x ⦂ T ∈ Γ ->
+      x ⦂ T ∈ Γ →
       {.free x}; Γ ⊢ x : T
-  |
+  | box [H : HasFeature i .box_type] : match i with
+          | .cc0 | .cc1 => ...
+          | .cc2 => ...
+          | .cc3 => by cases H
