CCDeconstructed/Var.lean
@@ -1,9 +1,11 @@
 import Mathlib.Data.Finset.Basic
 import Mathlib.Data.Finset.Lattice
+import Mathlib.Order.WithBot
+import Mathlib.Tactic.Ring
 
 import CCDeconstructed.CC
 
-inductive VarCat : CC -> Type where
+inductive VarCat : CC → Type where
   | var i : VarCat i
   | tvar i : VarCat i
   deriving Repr, DecidableEq
@@ -15,14 +17,45 @@ abbrev Index (_ : VarCat i) := Nat
 abbrev Atom (_ : VarCat i) := Nat
 
 namespace Atom
-  def freshFor (set : Finset (Atom α)) : ∃ (x : Atom α), x ∉ set := by
+  def list_max_or_0 (xs : List (Atom β)) : Atom β :=
+    xs.foldr (init := 0) max
+
+  lemma max_of_non_bot_is_not_bot (L : Finset (Atom β)) (x : Atom β) :
+    ¬(max (↑x) (Finset.max (Finset.erase L x)) = none)
+  := by
+    intros Eq
+    have h : @Nat.cast (WithBot (Atom β)) AddMonoidWithOne.toNatCast x ≤ none
+    := by
+      rw [<- Eq]
+      apply le_max_left
+    have xIsNone : @Nat.cast (WithBot (Atom β)) AddMonoidWithOne.toNatCast x = none
+    := le_bot_iff.mp h
+    injection xIsNone
+
+  def max_of_nonempty {L : Finset (Atom β)} (h : L.Nonempty) :
+    { x : Atom β // L.max = x }
+  := by
+    generalize Eq : Finset.max L = M
+    cases M
+    · case none =>
+      exfalso
+      let ⟨x, xIn⟩ := h
+      rw [<- Finset.insert_erase xIn] at Eq
+      rw [Finset.max_insert] at Eq
+      apply max_of_non_bot_is_not_bot
+      apply Eq
+    · case some x =>
+      apply Subtype.mk x
+      rfl
+
+  def freshFor (set : Finset (Atom α)) : { x : Atom α // x ∉ set } := by
     cases Finset.decidableNonempty
     · case isFalse notNonempty =>
       exists 0
       contrapose! notNonempty
       exists 0
     · case isTrue nonempty =>
-      cases Finset.max_of_nonempty nonempty
+      cases max_of_nonempty nonempty
       rename_i max eq
       exists max + 1
       apply Finset.not_mem_of_max_lt (b := max)
@@ -40,8 +73,8 @@ instance : DecidableEq (Atom α) := Atom.instDecidableEq
 
 @[aesop unsafe [constructors 10%,cases 20%]]
 inductive Var (α : VarCat i) : Type where
-  | free : Atom α -> Var α
-  | bound : Index α -> Var α
+  | free : Atom α → Var α
+  | bound : Index α → Var α
   | cap {_ : α = var i} : Var α
 
 instance : DecidableEq (Var α) := by
