CCDeconstructed/WellFormedness.lean
@@ -1,97 +1,356 @@
 import CCDeconstructed.Var
 import CCDeconstructed.Syntax
 import CCDeconstructed.CC
-import CCDeconstructed.Env
+import CCDeconstructed.Infrastructure
 
-open Feature VarCat
+open Feature VarCat Env
 
-variable {i : CC}
+set_option linter.unusedVariables false
 
 namespace Var
-  inductive WellFormed (Γ : Env i) : @Var i α -> Prop where
-    | freeVar : x ∈ Γ.dom (var i) -> WellFormed Γ (@Var.free i (var i) x)
-    | freeTVar : x ∈ Γ.dom (tvar i) -> WellFormed Γ (@Var.free i (tvar i) x)
-    | cap : WellFormed Γ .cap
+  def WellFormed {i : CC} {α : VarCat i} (allowCap := false) (Γ : Env i) : Var α → Prop
+    | .free x => x ∈ dom Γ
+    | .bound _ => False
+    | .cap => if allowCap then True else False
+
+  lemma WellFormed_WellScoped {α : VarCat i} (allowCap := false) {Γ : Env i} {v : Var α} :
+    WellFormed allowCap Γ v →
+    WellScoped allowCap v
+  := by cases v <;> simp [WellFormed,WellScoped]
+
+  @[aesop unsafe 40%]
+  lemma WellFormed_weaken {α : VarCat i} (allowCap := false) {Γ Δ : Env i} {v : Var α} :
+    WellFormed allowCap Δ v →
+    WellFormed allowCap (Γ ++ Δ) v
+  := by cases v <;> simp [WellFormed,Env.dom_concat]; aesop
+
+  instance instWellFormedness {α : VarCat i} (allowCap : Bool) : WellFormedness i (Var α) where
+    WellScoped := WellScoped allowCap
+    WellScopedRec := WellScopedRec allowCap
+    WellScoped_implies_WellScopedRec_0 := WellScoped_implies_WellScopedRec_0
+    WellScopedRec_weaken := WellScopedRec_weaken
+    WellFormed := WellFormed allowCap
+    WellFormed_WellScoped := WellFormed_WellScoped allowCap
+    WellFormed_weaken := WellFormed_weaken allowCap
 end Var
 
 namespace Cap
   def WellFormed (Γ : Env i) (C : Cap i) : Prop :=
-    ∀ v ∈ C, Var.WellFormed Γ v
+    ∀ v ∈ C, Var.WellFormed (allowCap := true) Γ v
+
+  lemma WellFormed_WellScoped :
+    Cap.WellFormed Γ C →
+    Cap.WellScoped C
+  := by
+    intros C.WF v v.In
+    eapply Var.WellFormed_WellScoped
+    apply C.WF; apply v.In
+
+  @[simp]
+  lemma WellFormed_empty :
+    WellFormed Γ ∅
+  := by simp [WellFormed]
+
+  lemma WellFormed_union :
+    WellFormed Γ C →
+    WellFormed Γ D →
+    WellFormed Γ (C ∪ D)
+  := by
+    simp [WellFormed]
+    aesop
+
+  @[aesop unsafe 40%]
+  lemma WellFormed_weaken :
+    WellFormed Δ C →
+    WellFormed (Γ ++ Δ) C
+  := fun WF v In => Var.WellFormed_weaken (allowCap := true) (WF v In)
+
+  instance instWellFormedness : WellFormedness i (Cap i) where
+    WellFormed := WellFormed
+    WellFormed_WellScoped := WellFormed_WellScoped
+    WellFormed_weaken := WellFormed_weaken
 end Cap
 
 mutual
-  inductive Typ.Type : Typ i -> Prop where
-    | shape : Shape S -> Typ.Type S
-    | cap : Shape S -> Cap.WellScoped C -> Typ.Type (.cap S C)
+  inductive Typ.Type : Typ i → Prop where
+    | shape : Shape S → Typ.Type S
+    | cap : Shape S → Cap.WellScoped C → Typ.Type (.cap S C)
 
-  inductive Typ.Shape : Typ i -> Prop where
+  inductive Typ.Shape : Typ i → Prop where
     | var : Shape (.var (.free X))
     | top : Shape top
     | arr (L : Finset (Atom (.var i))) :
-        Typ.Type T ->
-        (∀ x ∉ L, Typ.Type (@Scoped.instantiate _ _ (.var i) _ U (.free x))) ->
+        Typ.Type T →
+        (∀ x ∉ L, Typ.Type (Typ.instantiateRecVar U 0 (.free x))) →
         Typ.Shape (.arr T U)
     | all (L : Finset (Atom (.tvar i))) :
-        Typ.Shape S ->
-        (∀ X ∉ L, Typ.Type (@Scoped.instantiate _ _ (.tvar i) _ U (.var (.free X)))) ->
+        Typ.Shape S →
+        (∀ X ∉ L, Typ.Type (Typ.instantiateRecTyp U 0 (.var (.free X)))) →
         Typ.Shape (.all k T U)
     | box [HasFeature i box_type] :
-        Typ.Type T ->
-        Typ.Shape (.box T)
+        Typ.Type T →
+        Typ.Shape (@Typ.box i _ T)
 end
 
-inductive Typ.WellFormed : Env i -> Typ i -> Prop where
-  | var : X <: R ∈ Γ -> Typ.WellFormed Γ X
-  | top : Typ.WellFormed Γ .top
-  | arr (L : Finset (Atom (.var i))) :
-      Typ.WellFormed Γ T ->
-      (∀ x ∉ L, Typ.WellFormed (Γ ▷ x ⦂ T) (@Scoped.instantiate _ _ (.var i) _ U (.free x))) ->
-      Typ.WellFormed Γ (.arr T U)
-  | all (L : Finset (Atom (.tvar i))) :
-      Typ.WellFormed Γ S ->
-      Typ.Shape S ->
-      (∀ X ∉ L, Typ.WellFormed (Γ ▷ X <: S) (@Scoped.instantiate _ _ (.tvar i) _ U (.var (.free X)))) ->
-      Typ.WellFormed Γ (.all k S U)
-  | box :
-      Typ.WellFormed Γ T ->
-      Typ.WellFormed Γ (.box T)
-  | cap :
-      Typ.WellFormed Γ S ->
-      Typ.Shape S ->
-      Cap.WellFormed Γ C ->
-      Typ.WellFormed Γ (.cap S C)
+namespace Typ
+  inductive WellFormed : Env i → Typ i → Prop where
+    | var :
+        X <: S ∈ Γ →
+        WellFormed Γ X
+    | top : WellFormed Γ .top
+    | arr (L : Finset (Atom (.var i))) :
+        WellFormed Γ T →
+        (∀ x ∉ L, WellFormed (Γ ▷ x ⦂ T) (Typ.instantiateRecVar U 0 (.free x))) →
+        WellFormed Γ (.arr T U)
+    | all (L : Finset (Atom (.tvar i))) :
+        WellFormed Γ S →
+        Shape S →
+        (∀ X ∉ L, Typ.WellFormed (Γ ▷ X <: S) (Typ.instantiateRecTyp U 0 (.var (.free X)))) →
+        WellFormed Γ (.all k S U)
+    | box [HasFeature i box_type] :
+        WellFormed Γ T →
+        WellFormed Γ (@Typ.box i _ T)
+    | cap :
+        WellFormed Γ S →
+        Shape S →
+        Cap.WellFormed Γ C →
+        WellFormed Γ (.cap S C)
 
-inductive Env.WellFormed : Env i -> Prop where
+  lemma WellFormed_WellScoped :
+    WellFormed Γ T →
+    WellScoped T
+  := by
+    intros T.WF
+    induction T.WF
+    · case var X R Γ X.In =>
+      constructor; constructor
+    · case top Γ =>
+      constructor
+    · case arr Γ T U L T.WF U.WF T.IH U.IH =>
+      constructor
+      · exact T.IH
+      · exact U.IH
+    · case all Γ S U k L S.WF S.Shape U.WF S.WS U.IH =>
+      constructor
+      · exact S.WS
+      · exact U.IH
+    · case box Γ T _ T.WF T.IH =>
+      constructor; exact T.IH
+    · case cap Γ S C S.WF S.Shape C.WF S.WS =>
+      constructor
+      · exact S.WS
+      · apply Cap.WellFormed_WellScoped C.WF
+
+  lemma WellFormed_weaken :
+    WellFormed Δ T →
+    WellFormed (Γ ++ Δ) T
+  := by
+    rename_i i
+    intros WF
+    induction WF
+    · case var X T Δ X.Mem =>
+      apply WellFormed.var (S := T)
+      apply Env.mem_tail X.Mem
+    · case top => constructor
+    · case arr Δ T U L T.WF U.WF T.IH U.IH =>
+      apply WellFormed.arr L T.IH
+      intros x x.NotIn
+      rw [<- Env.concat_cons]
+      exact U.IH x x.NotIn
+    · case all Δ S U k L S.WF S.Shape U.WF S.IH U.IH =>
+      apply WellFormed.all L S.IH S.Shape
+      intros X X.NotIn
+      rw [<- Env.concat_cons]
+      exact U.IH X X.NotIn
+    · case box Δ T _ T.WF T.IH =>
+      apply WellFormed.box T.IH
+    · case cap Δ S C S.WF S.Shape C.WF S.IH =>
+      exact WellFormed.cap S.IH S.Shape (Cap.WellFormed_weaken C.WF)
+
+  lemma WellFormed_weaken_head :
+    a.name ∉ dom Γ →
+    WellFormed Γ T →
+    WellFormed (Γ ▷ a) T
+  := by
+    rename_i i
+    intros NotIn WF
+    induction WF
+    · case var X T Δ X.Mem =>
+      apply WellFormed.var (S := T)
+      apply Env.mem_cons_tail
+      · exact Γ
+      · simp
+        intros Eq
+        cases
+        apply HEq
+
+
+    · case top => constructor
+    · case arr Δ T U L T.WF U.WF T.IH U.IH =>
+      apply WellFormed.arr L T.IH
+      intros x x.NotIn
+      rw [<- Env.concat_cons]
+      exact U.IH x x.NotIn
+    · case all Δ S U k L S.WF S.Shape U.WF S.IH U.IH =>
+      apply WellFormed.all L S.IH S.Shape
+      intros X X.NotIn
+      rw [<- Env.concat_cons]
+      exact U.IH X X.NotIn
+    · case box Δ T _ T.WF T.IH =>
+      apply WellFormed.box T.IH
+    · case cap Δ S C S.WF S.Shape C.WF S.IH =>
+      exact WellFormed.cap S.IH S.Shape (Cap.WellFormed_weaken C.WF)
+
+  instance instWellFormedness : WellFormedness i (Typ i) where
+    WellFormed := WellFormed
+    WellFormed_WellScoped := WellFormed_WellScoped
+    WellFormed_weaken := WellFormed_weaken
+end Typ
+
+inductive Env.WellFormed : Env i → Prop where
   | nil : Env.WellFormed ∅
   | val :
-      Env.WellFormed Γ ->
-      Typ.WellFormed Γ T ->
+      Env.WellFormed (erase Γ x) →
+      Typ.WellFormed (erase Γ x) T →
       Env.WellFormed (Γ ▷ x ⦂ T)
-  | sub (S : Typ i) :
-      Env.WellFormed Γ ->
-      Typ.WellFormed Γ S ->
-      Env.WellFormed (Γ ▷ x <: S)
+  | sub :
+      Env.WellFormed (erase Γ X) →
+      Typ.WellFormed (erase Γ X) S →
+      Typ.Shape S →
+      Env.WellFormed (Γ ▷ X <: S)
   | typ [HasFeature i type_bindings] :
-      Env.WellFormed Γ ->
-      Typ.WellFormed Γ T ->
-      Env.WellFormed (Γ ▷ X ≔ T)
+      Env.WellFormed (erase Γ X) →
+      Typ.WellFormed (erase Γ X) T →
+      Env.WellFormed (Γ ▷ @Assoc.typ i _ X T)
 
-lemma Var.WellFormed_WellScoped :
-  Var.WellFormed Γ v ->
-  Var.WellScoped v
-:= by intros v.WF; cases v.WF <;> constructor
+namespace Env
+  @[elab_as_elim,eliminator]
+  lemma WellFormed.rec_bindings {i : CC} {motive : (Γ : Env i) → WellFormed Γ → Prop}
+    (nil : motive ∅ .nil)
+    (val : ∀ {Γ : Env i} {x : Atom (var i)} {T : Typ i}
+             (xNotIn : x ∉ dom Γ)
+             (ΓWF : WellFormed Γ)
+             (TWF : Typ.WellFormed Γ T),
+          motive Γ ΓWF →
+          motive (Γ ▷ x ⦂ T) (.val ((Env.erase_not_in_dom xNotIn).symm ▸ ΓWF)
+                                   ((Env.erase_not_in_dom xNotIn).symm ▸ TWF)))
+    (sub : ∀ {Γ : Env i} {X : Atom (tvar i)} {S : Typ i}
+             (XNotIn : X ∉ dom Γ)
+             (ΓWF : WellFormed Γ)
+             (SWF : Typ.WellFormed Γ S)
+             (SShape : Typ.Shape S),
+          motive Γ ΓWF →
+          motive (Γ ▷ X <: S) (.sub ((Env.erase_not_in_dom XNotIn).symm ▸ ΓWF)
+                                    ((Env.erase_not_in_dom XNotIn).symm ▸ SWF)
+                                    SShape))
+    (typ : ∀ {Γ : Env i} {X : Atom (tvar i)} {T : Typ i}
+             (XNotIn : X ∉ dom Γ)
+             (ΓWF : WellFormed Γ)
+             (TWF : Typ.WellFormed Γ T),
+          motive Γ ΓWF →
+          motive (Γ ▷ X ≔ T) (.typ ((Env.erase_not_in_dom XNotIn).symm ▸ ΓWF)
+                                   ((Env.erase_not_in_dom XNotIn).symm ▸ TWF)))
+    : ∀ {Γ : Env i} (ΓWF : WellFormed Γ), motive Γ ΓWF
+  := by
+    intros Γ ΓWF
+    induction Γ
+    · case nil =>
+      apply nil
+    · case val x T Γ x.NotIn IH =>
+      generalize Eq.gen : Γ ▷ x ⦂ T = Δ at ΓWF
+      cases ΓWF
+      · case nil => simp [Env.cons_not_nil] at Eq.gen
+      · case val Γ' x' T' Γ'.WF T'.WF =>
+        obtain ⟨Eq.Γ, Eq.a⟩ := Env.cons_eq_iff.mp Eq.gen
+        simp [Env.erase_not_in_dom x.NotIn] at Eq.Γ
+        simp at Eq.a
+        obtain ⟨Eq.x, Eq.T⟩ := Eq.a
+        conv =>
+          lhs
+          rw [<- Eq.gen]
+          rfl
+        rw [<- Eq.Γ] at Γ'.WF T'.WF
+        rw [<- Eq.T] at T'.WF
+        apply val x.NotIn Γ'.WF T'.WF (IH Γ'.WF)
+      · case sub =>
+        obtain ⟨Eq.Γ, Eq.a⟩ := Env.cons_eq_iff.mp Eq.gen
+        simp at Eq.a
+      · case typ =>
+        obtain ⟨Eq.Γ, Eq.a⟩ := Env.cons_eq_iff.mp Eq.gen
+        simp at Eq.a
+    · case sub X S Γ X.NotIn IH =>
+      generalize Eq.gen : Γ ▷ X <: S = Δ at ΓWF
+      cases ΓWF
+      · case nil => simp [Env.cons_not_nil] at Eq.gen
+      · case val =>
+        obtain ⟨Eq.Γ, Eq.a⟩ := Env.cons_eq_iff.mp Eq.gen
+        simp at Eq.a
+      · case sub Γ' X' S' Γ'.WF S'.WF S'.Shape =>
+        obtain ⟨Eq.Γ, Eq.a⟩ := Env.cons_eq_iff.mp Eq.gen
+        simp [Env.erase_not_in_dom X.NotIn] at Eq.Γ
+        simp at Eq.a
+        obtain ⟨Eq.X, Eq.S⟩ := Eq.a
+        conv =>
+          lhs
+          rw [<- Eq.gen]
+          rfl
+        rw [<- Eq.Γ] at Γ'.WF S'.WF
+        rw [<- Eq.S] at S'.WF S'.Shape
+        apply sub X.NotIn Γ'.WF S'.WF S'.Shape (IH Γ'.WF)
+      · case typ =>
+        obtain ⟨Eq.Γ, Eq.a⟩ := Env.cons_eq_iff.mp Eq.gen
+        simp at Eq.a
+    · case typ X T Γ X.NotIn IH =>
+      generalize Eq.gen : Γ ▷ X ≔ T = Δ at ΓWF
+      cases ΓWF
+      · case nil => simp [Env.cons_not_nil] at Eq.gen
+      · case val =>
+        obtain ⟨Eq.Γ, Eq.a⟩ := Env.cons_eq_iff.mp Eq.gen
+        simp at Eq.a
+      · case sub =>
+        obtain ⟨Eq.Γ, Eq.a⟩ := Env.cons_eq_iff.mp Eq.gen
+        simp at Eq.a
+      · case typ Γ' T' X' _ Γ'.WF T'.WF =>
+        obtain ⟨Eq.Γ, Eq.a⟩ := Env.cons_eq_iff.mp Eq.gen
+        simp [Env.erase_not_in_dom X.NotIn] at Eq.Γ
+        simp at Eq.a
+        obtain ⟨Eq.X, Eq.T⟩ := Eq.a
+        conv =>
+          lhs
+          rw [<- Eq.gen]
+          rfl
+        rw [<- Eq.Γ] at Γ'.WF T'.WF
+        rw [<- Eq.T] at T'.WF
+        apply typ X.NotIn Γ'.WF T'.WF (IH Γ'.WF)
+      · case sub =>
+        obtain ⟨Eq.Γ, Eq.a⟩ := Env.cons_eq_iff.mp Eq.gen
+        simp at Eq.a
+      · case typ =>
+        obtain ⟨Eq.Γ, Eq.a⟩ := Env.cons_eq_iff.mp Eq.gen
+        simp at Eq.a
 
-lemma Cap.WellFormed_WellScoped :
-  Cap.WellFormed Γ C ->
-  Cap.WellScoped C
-:= by
-  intros C.WF v v.In
-  eapply Var.WellFormed_WellScoped
-  apply C.WF; apply v.In
+  lemma WellFormed_of_mem {Γ : Env i} :
+    Env.WellFormed Γ →
+    a ∈ Γ →
+    Typ.WellFormed Γ a.type
+  := by
+    intros Γ.WF a.In
+    induction Γ.WF
+    · case nil => simp [Env.not_mem_nil] at a.In
+    all_goals {
+      rename_i Γ x T x.NotIn Γ.WF T.WF Γ.IH
+      simp [Env.mem_cons] at a.In
+      rw [Env.erase_not_in_dom x.NotIn] at a.In
+      cases a.In
+      · case inl a.In =>
+        apply WellFormedness.WellFormed_weaken_head
+        sorry
+    }
+end Env
 
 lemma Typ.WellFormed_Type :
-  Env.WellFormed Γ ->
-  Typ.WellFormed Γ T ->
+  Env.WellFormed Γ →
+  Typ.WellFormed Γ T →
   Typ.Type T
 := by
   intros Γ.WF T.WF
