CCDeconstructed/Bisimulation.lean
@@ -4,4 +4,4 @@ structure State (i : CC) where
   store : Env
 
 class Eval (i : CC) where
-  Eval : State i -> State i -> Prop
+  Eval : State i → State i → Prop
