CCDeconstructed/Infrastructure/Cap.lean
@@ -1,0 +1,128 @@
+import CCDeconstructed.Syntax
+import CCDeconstructed.Classes
+import CCDeconstructed.Infrastructure.Var
+
+open Scoped FreeVariables VarCat
+
+namespace Cap
+  @[aesop norm]
+  def fv (C : Cap i) : Finset (Atom (var i)) :=
+    C.fold (· ∪ ·) ∅ Var.fv
+
+  lemma mem_free_iff_mem_fv :
+    .free x ∈ C ↔ x ∈ fv C
+  := by
+    induction' C using Finset.induction <;> aesop
+
+  @[aesop safe apply]
+  lemma mem_free_implies_mem_fv :
+    .free x ∈ C → x ∈ fv C
+  := Iff.mp mem_free_iff_mem_fv
+
+  lemma mem_fv_implies_mem_free :
+    x ∈ fv C → .free x ∈ C
+  := Iff.mpr mem_free_iff_mem_fv
+
+  @[aesop norm]
+  def bv (C : Cap i) : Finset (Index (var i)) :=
+    C.fold (· ∪ ·) ∅ Var.bv
+
+  lemma mem_bound_iff_mem_bv :
+    .bound k ∈ C ↔ k ∈ bv C
+  := by
+    induction' C using Finset.induction <;> aesop
+
+  @[aesop safe apply]
+  lemma mem_bound_implies_mem_bv :
+    .bound k ∈ C → k ∈ bv C
+  := Iff.mp mem_bound_iff_mem_bv
+
+  lemma mem_bv_implies_mem_bound :
+    k ∈ bv C → .bound k ∈ C
+  := Iff.mpr mem_bound_iff_mem_bv
+
+  instance : FreeVariables (Cap i) (var i) where
+    fv := fv
+
+  @[aesop norm 10]
+  def instantiateRec (C : Cap i) (k : Index (var i)) (u : Var (var i)) :=
+    if .bound k ∈ C then
+      C \ {.bound k} ∪ {u}
+    else
+      C
+
+  @[aesop norm 10]
+  def substitute (C : Cap i) (x : Atom (var i)) (u : Var (var i)) :=
+    if .free x ∈ C then
+      C \ {.free x} ∪ {u}
+    else
+      C
+
+  @[aesop norm 5]
+  def WellScopedRec (n : Nat) (C : Cap i) :=
+    ∀ v ∈ C, Var.WellScopedRec (allowCap := true) n v
+
+  @[aesop norm 5]
+  def WellScoped (C : Cap i) :=
+    ∀ v ∈ C, Var.WellScoped (allowCap := true) v
+
+  @[aesop safe forward]
+  lemma WellScoped_implies_WellScopedRec_0 :
+    WellScoped C →
+    WellScopedRec 0 C
+  := by aesop
+
+  @[simp,aesop safe forward]
+  lemma WellScopedRec_weaken :
+    m <= n →
+    WellScopedRec m C →
+    WellScopedRec n C
+  := by
+    intros leq C.WS v v.In
+    apply Var.WellScopedRec_weaken <;> aesop
+
+  instance instWellScopedness : WellScopedness (Cap i) where
+    WellScopedRec := WellScopedRec
+    WellScoped := WellScoped
+    WellScoped_implies_WellScopedRec_0 := WellScoped_implies_WellScopedRec_0
+    WellScopedRec_weaken := WellScopedRec_weaken
+
+  lemma substitute_fresh :
+    x ∉ fv C →
+    substitute C x u = C
+  := by
+    simp [substitute]
+    intros x.NotIn x.In
+    exfalso; apply x.NotIn
+    apply mem_free_implies_mem_fv x.In
+
+  @[simp]
+  lemma WellScopedRec_instantiateRec :
+    WellScopedRec n (instantiateRec C n u) →
+    WellScopedRec (n + 1) C
+  := by
+    intros C.WS v v.WS
+    apply Var.WellScopedRec_instantiateRec (u := u)
+    apply C.WS
+    simp only [instantiateRec]
+    aesop
+
+  @[simp]
+  lemma instantiateRec_WellScopedRec :
+    WellScopedRec n C →
+    k >= n →
+    instantiateRec C k u = C
+  := by aesop
+
+  @[simp]
+  instance instScoped : Scoped (Cap i) (var i) where
+    instantiateRec := instantiateRec
+    substitute := substitute
+    substitute_fresh := substitute_fresh
+    WellScopedRec_instantiateRec := WellScopedRec_instantiateRec
+    instantiateRec_WellScopedRec := instantiateRec_WellScopedRec
+
+  instance instEmptyCollection : EmptyCollection (Cap i) := inferInstance
+  instance instSingleton : Singleton (Var (.var i)) (Cap i) := inferInstance
+  instance instMembership : Membership (Var (.var i)) (Cap i) := inferInstance
+end Cap
