CCDeconstructed/Infrastructure/Env.lean
@@ -1,0 +1,85 @@
+import CCDeconstructed.Syntax
+import CCDeconstructed.Classes
+import CCDeconstructed.Tactics
+import CCDeconstructed.Infrastructure.Typ
+
+set_option linter.unusedVariables false
+
+open Scoped FreeVariables VarCat
+
+namespace Binder
+  instance instFreeVariables {α : VarCat i} : FreeVariables (Binder i) α where
+    fv := Binder.dom
+end Binder
+
+namespace Assoc
+  def freeVariables {α : VarCat i} (a : Assoc i) : Finset (Atom α) :=
+    match α with
+    | .var _ => Typ.freeVariablesVar (Assoc.type a)
+    | .tvar _ => Typ.freeVariablesTyp (Assoc.type a)
+
+  instance instFreeVariables {α : VarCat i} : FreeVariables (Assoc i) α where
+    fv := freeVariables
+
+  @[simp]
+  def WellScopedRec (n : Nat) (a : Assoc i) : Prop :=
+    Typ.WellScopedRec n (type a)
+
+  @[simp]
+  def WellScoped (a : Assoc i) : Prop :=
+    Typ.WellScoped (type a)
+
+  lemma WellScoped_implies_WellScopedRec_0 :
+    WellScoped a →
+    WellScopedRec 0 a
+  := by
+    simp [type]
+    cases a <;> simp <;> apply Typ.WellScoped_implies_WellScopedRec_0
+
+  lemma WellScopedRec_weaken :
+    m ≤ n →
+    WellScopedRec m a →
+    WellScopedRec n a
+  := by
+    simp [type]
+    cases a <;> simp <;> apply Typ.WellScopedRec_weaken
+
+  instance instWellScopedness : WellScopedness (Assoc i) where
+    WellScopedRec := WellScopedRec
+    WellScoped := WellScoped
+    WellScoped_implies_WellScopedRec_0 := WellScoped_implies_WellScopedRec_0
+    WellScopedRec_weaken := WellScopedRec_weaken
+end Assoc
+
+namespace Env
+  def freeVariables {α : VarCat i} (Γ : Env i) : Finset (Atom α) :=
+    List.foldr (init := ∅) (Assoc.freeVariables · ∪ ·) Γ.assocs
+
+  instance instFreeVariables {α : VarCat i} : FreeVariables (Env i) α where
+    fv := freeVariables
+
+  @[simp]
+  def WellScopedRec (n : Nat) (Γ : Env i) : Prop :=
+    Γ.assocs.Forall (Assoc.WellScopedRec n)
+
+  @[simp]
+  def WellScoped (Γ : Env i) : Prop :=
+    Γ.assocs.Forall Assoc.WellScoped
+
+  lemma WellScoped_implies_WellScopedRec_0 :
+    WellScoped Γ →
+    WellScopedRec 0 Γ
+  := List.Forall.imp (@Assoc.WellScoped_implies_WellScopedRec_0 _)
+
+  lemma WellScopedRec_weaken :
+    m ≤ n →
+    WellScopedRec m a →
+    WellScopedRec n a
+  := fun leq => List.Forall.imp (fun _ WS => Assoc.WellScopedRec_weaken leq WS)
+
+  instance instWellScopedness : WellScopedness (Env i) where
+    WellScopedRec := WellScopedRec
+    WellScoped := WellScoped
+    WellScoped_implies_WellScopedRec_0 := WellScoped_implies_WellScopedRec_0
+    WellScopedRec_weaken := WellScopedRec_weaken
+end Env
