CCDeconstructed/Infrastructure/Exp.lean
@@ -1,0 +1,552 @@
+import CCDeconstructed.Syntax
+import CCDeconstructed.Classes
+import CCDeconstructed.Tactics
+import CCDeconstructed.Infrastructure.Var
+import CCDeconstructed.Infrastructure.Typ
+
+set_option linter.unusedVariables false
+
+open Scoped FreeVariables VarCat
+
+namespace Exp
+  instance : Coe (Var (.var i)) (Exp i) where
+    coe := Exp.var
+
+  @[aesop norm]
+  def freeVariablesVar (e : Exp i) : Finset (Atom (.var i)) :=
+    match e with
+    | .var v => v.fv
+    | .abs _ e => e.freeVariablesVar
+    | .app f e => f.fv ∪ e.fv
+    | .tabs _ e => e.freeVariablesVar
+    | .tapp f _ => f.fv
+    | .let_ e1 e2 => e1.freeVariablesVar ∪ e2.freeVariablesVar
+    | @Exp.type _ _ _ e => e.freeVariablesVar
+    | @Exp.box _ _ x => x.fv
+    | @Exp.unbox _ _ x => x.fv
+
+  @[aesop norm]
+  def freeVariablesTyp (e : Exp i) : Finset (Atom (.tvar i)) :=
+    match e with
+    | .var _ => ∅
+    | .abs T e => T.freeVariablesTyp ∪ e.freeVariablesTyp
+    | .app _ _ => ∅
+    | .tabs T e => T.freeVariablesTyp ∪ e.freeVariablesTyp
+    | .tapp _ T => T.freeVariablesTyp
+    | .let_ e1 e2 => e1.freeVariablesTyp ∪ e2.freeVariablesTyp
+    | @Exp.type _ _ T e => T.freeVariablesTyp ∪ e.freeVariablesTyp
+    | @Exp.box _ _ _ => ∅
+    | @Exp.unbox _ _ _ => ∅
+
+  instance : FreeVariables (Exp i) (.var i) where
+    fv := freeVariablesVar
+
+  instance : FreeVariables (Exp i) (.tvar i) where
+    fv := freeVariablesTyp
+
+  @[aesop norm]
+  def instantiateRecVar (e : Exp i) (k : Index (.var i)) (u : Var (.var i)) : Exp i :=
+    match e with
+    | .var v => v.instantiateRec k u
+    | .abs T e => .abs T (e.instantiateRecVar (k + 1) u)
+    | .app f e => .app (f.instantiateRec k u) (e.instantiateRec k u)
+    | .tabs T e => .tabs T (e.instantiateRecVar (k + 1) u)
+    | .tapp x T => .tapp (x.instantiateRec k u) T
+    | .let_ e1 e2 => .let_ (e1.instantiateRecVar k u) (e2.instantiateRecVar (k + 1) u)
+    | @Exp.type _ _ T e => .type T (e.instantiateRecVar (k + 1) u)
+    | @Exp.box _ _ x => .box (x.instantiateRec k u)
+    | @Exp.unbox _ _ x => .unbox (x.instantiateRec k u)
+
+  @[aesop norm]
+  def substituteVar (e : Exp i) (x : Atom (.var i)) (u : Var (.var i)) : Exp i :=
+    match e with
+    | .var v => v.substitute x u
+    | .abs T e => .abs T (e.substituteVar x u)
+    | .app f e =>.app (f.substitute x u) (e.substitute x u)
+    | .tabs T e => .tabs T (e.substituteVar x u)
+    | .tapp f T => .tapp (f.substitute x u) T
+    | .let_ e1 e2 => .let_ (e1.substituteVar x u) (e2.substituteVar x u)
+    | @Exp.type _ _ T e => .type T (e.substituteVar x u)
+    | @Exp.box _ _ v => .box (v.substitute x u)
+    | @Exp.unbox _ _ v => .unbox (v.substitute x u)
+
+  @[aesop norm]
+  def instantiateRecTyp (e : Exp i) (K : Index (.tvar i)) (U : Typ i) : Exp i :=
+    match e with
+    | .var v => v
+    | .abs T e => .abs (T.instantiateRecTyp K U) (e.instantiateRecTyp (K + 1) U)
+    | .app f e =>.app f e
+    | .tabs T e => .tabs (T.instantiateRecTyp K U) (e.instantiateRecTyp (K + 1) U)
+    | .tapp f T => .tapp f (T.instantiateRecTyp K U)
+    | .let_ e1 e2 => .let_ (e1.instantiateRecTyp K U) (e2.instantiateRecTyp (K + 1) U)
+    | @Exp.type _ _ T e => .type (T.instantiateRecTyp K U) (e.instantiateRecTyp (K + 1) U)
+    | @Exp.box _ _ x => .box x
+    | @Exp.unbox _ _ x => .unbox x
+
+  @[aesop norm]
+  def substituteTyp (e : Exp i) (X : Atom (.tvar i)) (U : Typ i) : Exp i :=
+    match e with
+    | .var v => .var v
+    | .abs T e => .abs (T.substituteTyp X U) (e.substituteTyp X U)
+    | .app f e =>.app f e
+    | .tabs T e => .tabs (T.substituteTyp X U) (e.substituteTyp X U)
+    | .tapp f T => .tapp f (T.substituteTyp X U)
+    | .let_ e1 e2 => .let_ (e1.substituteTyp X U) (e2.substituteTyp X U)
+    | @Exp.type _ _ T e => .type (T.substituteTyp X U) (e.substituteTyp X U)
+    | @Exp.box _ _ x => .box x
+    | @Exp.unbox _ _ x => .unbox x
+
+  @[aesop unsafe constructors 50%]
+  inductive WellScopedRec {i : CC} : Nat → Exp i → Prop :=
+    | var :
+        Var.WellScopedRec (allowCap := false) n v →
+        WellScopedRec n (.var v)
+    | abs :
+        Typ.WellScopedRec n T →
+        WellScopedRec (n + 1) e →
+        WellScopedRec n (.abs T e)
+    | app :
+        Var.WellScopedRec (allowCap := false) n f →
+        Var.WellScopedRec (allowCap := false) n e →
+        WellScopedRec n (.app f e)
+    | tabs :
+        Typ.WellScopedRec n T →
+        WellScopedRec (n + 1) e →
+        WellScopedRec n (.tabs T e)
+    | tapp :
+        Var.WellScopedRec (allowCap := false) n f →
+        Typ.WellScopedRec n T →
+        WellScopedRec n (.tapp f T)
+    | let_ :
+        WellScopedRec n e1 →
+        WellScopedRec (n + 1) e2 →
+        WellScopedRec n (.let_ e1 e2)
+    | type [HasFeature i .type_bindings] :
+       Typ.WellScopedRec n T →
+       WellScopedRec (n + 1) e →
+       WellScopedRec n (.type T e)
+    | box [HasFeature i .explicit_boxing] :
+       Var.WellScopedRec (allowCap := false) n v →
+       WellScopedRec n (.box v)
+    | unbox [HasFeature i .explicit_boxing] :
+       Var.WellScopedRec (allowCap := false) n v →
+      WellScopedRec n (.unbox v)
+
+  @[aesop unsafe constructors 50%]
+  inductive WellScoped {i : CC} : Exp i → Prop :=
+    | var :
+        Var.WellScoped (allowCap := false) v →
+        WellScoped (.var v)
+    | abs (L : Finset (Atom (.var i))) :
+        Typ.WellScoped T →
+        (∀ x ∉ L, WellScoped (e.instantiateRecVar 0 x)) →
+        WellScoped (.abs T e)
+    | app :
+        Var.WellScoped (allowCap := false) f →
+        Var.WellScoped (allowCap := false) e →
+        WellScoped (.app f e)
+    | tabs (L : Finset (Atom (.tvar i))) :
+        Typ.WellScoped T →
+        (∀ X ∉ L, WellScoped (e.instantiateRecTyp 0 X)) →
+        WellScoped (.tabs T e)
+    | tapp :
+        Var.WellScoped (allowCap := false) f →
+        Typ.WellScoped T →
+        WellScoped (.tapp f T)
+    | let_ (L : Finset (Atom (.var i))) :
+        WellScoped e1 →
+        (∀ x ∉ L, WellScoped (e2.instantiateRecVar 0 x)) →
+        WellScoped (.let_ e1 e2)
+    | type [HasFeature i .type_bindings] (L : Finset (Atom (.tvar i))) :
+        Typ.WellScoped T →
+        (∀ X ∉ L, WellScoped (e.instantiateRecTyp 0 X)) →
+        WellScoped (.type T e)
+    | box [HasFeature i .explicit_boxing] :
+        Var.WellScoped (allowCap := false) v →
+        WellScoped (.box v)
+    | unbox [HasFeature i .explicit_boxing] :
+        Var.WellScoped (allowCap := false) v →
+        WellScoped (.unbox v)
+
+  @[elab_as_elim]
+  lemma WellScoped.locally_nameless_rec {i : CC}
+    {motive : ∀ (e : Exp i), WellScoped e → Prop}
+    (var : ∀ (x : Atom (.var i)), motive (.var x) (.var True.intro))
+    (abs : ∀ (T : Typ i) (e : Exp i) (L : Finset (Atom (.var i))) (x : Atom (.var i)) (xFresh : x ∉ L ∪ Typ.freeVariablesVar T ∪ freeVariablesVar e),
+      ∀ (TWS : Typ.WellScoped T)
+        (eWS : ∀ x ∉ L, WellScoped (e.instantiateRecVar 0 x))
+        (eIH : motive (instantiateRecVar e 0 x) (eWS x (by aesop))),
+      motive (.abs T e) (.abs L TWS eWS))
+    (app : ∀ (f e : Atom (.var i)),
+      motive (.app f e) (.app True.intro True.intro))
+    (tabs : ∀ (T : Typ i) (e : Exp i) (L : Finset (Atom (.tvar i))) (X : Atom (.tvar i)) (XFresh : X ∉ L ∪ Typ.freeVariablesTyp T ∪ freeVariablesTyp e),
+      ∀ (TWS : Typ.WellScoped T)
+        (eWS : ∀ X ∉ L, WellScoped (e.instantiateRecTyp 0 X))
+        (eIH : motive (instantiateRecTyp e 0 X) (eWS X (by aesop))),
+      motive (.tabs T e) (.tabs L TWS eWS))
+    (tapp : ∀ (f : Atom (.var i)) (T : Typ i),
+      ∀ (TWS : Typ.WellScoped T),
+      motive (.tapp f T) (.tapp True.intro TWS))
+    (let_ : ∀ (e1 : Exp i) (e2 : Exp i) (L : Finset (Atom (.var i))) (x : Atom (.var i)) (xFresh : x ∉ L ∪ freeVariablesVar e1 ∪ freeVariablesVar e2),
+      ∀ (e1WS : WellScoped e1)
+        (e2WS : ∀ x ∉ L, WellScoped (e2.instantiateRecVar 0 x))
+        (e1IH : motive e1 e1WS)
+        (e2IH : motive (instantiateRecVar e2 0 x) (e2WS x (by aesop))),
+      motive (.let_ e1 e2) (.let_ L e1WS e2WS))
+    (type : ∀ [HasFeature i .type_bindings] (T : Typ i) (e : Exp i) (L : Finset (Atom (.tvar i))) (X : Atom (.tvar i)) (XFresh : X ∉ L ∪ Typ.freeVariablesTyp T ∪ freeVariablesTyp e),
+      ∀ (TWS : Typ.WellScoped T)
+        (eWS : ∀ X ∉ L, WellScoped (e.instantiateRecTyp 0 X))
+        (eIH : motive (e.instantiateRecTyp 0 X) (eWS X (by aesop))),
+      motive (.type T e) (.type L TWS eWS))
+    (box : ∀ [HasFeature i .explicit_boxing] (x : Atom (.var i)),
+      motive (.box x) (.box True.intro))
+    (unbox : ∀ [HasFeature i .explicit_boxing] (x : Atom (.var i)),
+      motive (.unbox x) (.unbox True.intro))
+    : ∀ {e} WS, motive e WS
+  := by
+    intros e e.WS
+    induction e.WS
+    · case var v v.WS =>
+      cases v <;> simp [Var.WellScoped] at v.WS; apply var
+    · case abs T e L T.WS e.WS e.IH =>
+      pick_fresh x : .var i
+      apply abs T e _ x
+      · apply T.WS
+      · apply e.IH
+      · clear * - x.Fresh; aesop
+    · case app f e f.WS e.WS =>
+      cases f <;> cases e <;> simp [Var.WellScoped] at f.WS e.WS
+      rename_i f e
+      apply app
+    · case tabs T e L T.WS e.WS e.IH =>
+      pick_fresh X : .tvar i
+      apply tabs T e _ X
+      · apply T.WS
+      · apply e.IH
+      · clear * - X.Fresh; aesop
+    · case tapp f T f.WS T.WS =>
+      cases f <;> simp [Var.WellScoped] at f.WS
+      rename_i f
+      apply tapp
+      exact T.WS
+    · case let_ e1 e2 L e1.WS e2.WS e1.IH e2.IH =>
+      pick_fresh x : .var i
+      apply let_ e1 e2 _ x
+      · apply e1.IH
+      · apply e2.IH
+      · clear * - x.Fresh; aesop
+    · case type T e _ L T.WS e.WS e.IH =>
+      pick_fresh X : .tvar i
+      apply type T e _ X
+      · apply T.WS
+      · apply e.IH
+      · clear * - X.Fresh; aesop
+    · case box v _ v.WS =>
+      cases v <;> simp [Var.WellScoped] at v.WS
+      rename_i x
+      apply box
+    · case unbox v _ v.WS =>
+      cases v <;> simp [Var.WellScoped] at v.WS
+      rename_i x
+      apply unbox
+
+  @[aesop safe forward]
+  lemma WellScopedRec_instantiateRecTyp :
+    WellScopedRec n (e.instantiateRecTyp n U) →
+    WellScopedRec (n + 1) e
+  := by
+    intros e.WS
+    generalize Eq : instantiateRecTyp e n U = e'
+    rw [Eq] at e.WS
+    induction' e.WS generalizing e U
+    · case var n v v.WS =>
+      cases e <;> simp [instantiateRecTyp] at Eq
+      case var w =>
+      rw [Eq] at *
+      constructor
+      apply Var.WellScopedRec_weaken (m := n)
+      · linarith
+      · assumption
+    · case abs n T e1 T.WS _ e1.IH =>
+      cases e <;> simp [instantiateRecTyp] at Eq
+      case abs T' e' =>
+      rw [<- Eq.1] at T.WS
+      constructor
+      · apply Typ.WellScopedRec_instantiateRecTyp (U := U)
+        assumption
+      · apply e1.IH (U := U)
+        exact Eq.2
+    · case app n f e f.WS e.WS =>
+      cases e <;> simp [instantiateRecTyp] at Eq
+      case app n f' e' =>
+      constructor
+        <;> apply Var.WellScopedRec_weaken (m := n) (by linarith)
+        <;> rw [Eq.1,Eq.2] at *
+        <;> assumption
+    · case tabs n T e1 T.WS _ e1.IH =>
+      cases e <;> simp [instantiateRecTyp] at Eq
+      case tabs T' e' =>
+      rw [<- Eq.1] at T.WS
+      constructor
+      · apply Typ.WellScopedRec_instantiateRecTyp (U := U)
+        assumption
+      · apply e1.IH (U := U)
+        exact Eq.2
+    · case tapp n f T f.WS T.WS =>
+      cases e <;> simp [instantiateRecTyp] at Eq
+      case tapp n f' T' =>
+      constructor
+      · apply Var.WellScopedRec_weaken (m := n) (by linarith)
+        rw [Eq.1]
+        assumption
+      · apply Typ.WellScopedRec_instantiateRecTyp (U := U)
+        rw [Eq.2]
+        assumption
+    · case let_ n _ _ e1.WS e2.WS =>
+      cases e <;> simp [instantiateRecTyp] at Eq
+      case let_ n e1' e2' =>
+      constructor
+      · apply e1.WS Eq.1
+      · apply e2.WS Eq.2
+    · case type T e _ T.WS e.WS e.IH =>
+      cases e <;> simp [instantiateRecTyp] at Eq
+      case type T' e' =>
+      constructor
+      · apply Typ.WellScopedRec_instantiateRecTyp (U := U)
+        rw [Eq.1]
+        assumption
+      · apply e.IH (U := U)
+        exact Eq.2
+    · case box n v _ v.WS =>
+      cases e <;> simp [instantiateRecTyp] at Eq
+      case box w =>
+      rw [Eq] at *
+      constructor
+      apply Var.WellScopedRec_weaken (m := n) (by linarith) v.WS
+    · case unbox n v _ v.WS =>
+      cases e <;> simp [instantiateRecTyp] at Eq
+      case unbox w =>
+      rw [Eq] at *
+      constructor
+      apply Var.WellScopedRec_weaken (m := n) (by linarith) v.WS
+
+  @[aesop safe forward]
+  lemma WellScopedRec_instantiateRecVar :
+    WellScopedRec n (instantiateRecVar e n u) →
+    WellScopedRec (n + 1) e
+  := by
+    intros e.WS
+    generalize Eq : instantiateRecVar e n u = e'
+    rw [Eq] at e.WS
+    induction' e.WS generalizing e
+    · case var n v v.WS =>
+      cases e <;> simp [instantiateRecVar] at Eq
+      case var w =>
+      constructor
+      apply Var.WellScopedRec_instantiateRec (u := u)
+      rw [<- Eq] at v.WS
+      exact v.WS
+    · case abs n T e1 T.WS _ e1.IH =>
+      cases e <;> simp [instantiateRecVar] at Eq
+      case abs T' e' =>
+      rw [<- Eq.1] at T.WS
+      constructor
+      · apply Typ.WellScopedRec_weaken (m := n) (by linarith) T.WS
+      · apply e1.IH
+        exact Eq.2
+    · case app n f e f.WS e.WS =>
+      cases e <;> simp [instantiateRecVar] at Eq
+      case app n f' e' =>
+      constructor
+        <;> apply Var.WellScopedRec_instantiateRec (u := u)
+        <;> rw [Eq.1,Eq.2] at *
+        <;> assumption
+    · case tabs n T e1 T.WS _ e1.IH =>
+      cases e <;> simp [instantiateRecVar] at Eq
+      case tabs T' e' =>
+      constructor
+      · apply Typ.WellScopedRec_weaken (m := n) (by linarith)
+        rw [Eq.1]
+        exact T.WS
+      · apply e1.IH
+        exact Eq.2
+    · case tapp n f T f.WS T.WS =>
+      cases e <;> simp [instantiateRecVar] at Eq
+      case tapp n f' T' =>
+      constructor
+      · apply Var.WellScopedRec_instantiateRec (u := u)
+        rw [Eq.1]
+        exact f.WS
+      · apply Typ.WellScopedRec_weaken (m := n) (by linarith)
+        rw [Eq.2]
+        exact T.WS
+    · case let_ n _ _ e1.WS e2.WS =>
+      cases e <;> simp [instantiateRecVar] at Eq
+      case let_ e1' e2' =>
+      constructor
+      · apply e1.WS Eq.1
+      · apply e2.WS Eq.2
+    · case type n _ _ _ T.WS e.WS e.IH =>
+      cases e <;> simp [instantiateRecVar] at Eq
+      case type T' e' =>
+      constructor
+      · apply Typ.WellScopedRec_weaken (m := n) (by linarith)
+        rw [Eq.1]
+        exact T.WS
+      · apply e.IH
+        exact Eq.2
+    · case box n _ _ v.WS =>
+      cases e <;> simp [instantiateRecVar] at Eq
+      case box w =>
+      constructor
+      apply Var.WellScopedRec_instantiateRec (u := u)
+      rw [Eq]
+      exact v.WS
+    · case unbox n _ _ v.WS =>
+      cases e <;> simp [instantiateRecVar] at Eq
+      case unbox w =>
+      constructor
+      apply Var.WellScopedRec_instantiateRec (u := u)
+      rw [Eq]
+      exact v.WS
+
+  @[aesop safe forward]
+  lemma WellScoped_implies_WellScopedRec_0 :
+    WellScoped e →
+    WellScopedRec 0 e
+  := by
+    intros WS
+    induction' WS <;> constructor <;> aesop
+
+  @[aesop safe forward]
+  lemma WellScopedRec_weaken :
+    m <= n →
+    WellScopedRec m e→
+    WellScopedRec n e
+  := by
+    intros leq WS
+    induction' WS generalizing n
+    · case var m v v.WS =>
+      constructor
+      apply Var.WellScopedRec_weaken (m := m) leq v.WS
+    · case abs m T e T.WS e.WS e.IH =>
+      constructor
+      · apply Typ.WellScopedRec_weaken (m := m) leq T.WS
+      · apply e.IH; linarith
+    · case app m f e f.WS e.WS =>
+      constructor
+        <;> apply Var.WellScopedRec_weaken (m := m) leq
+        <;> assumption
+    · case tabs m T e T.WS e.WS e.IH =>
+      constructor
+      · apply Typ.WellScopedRec_weaken (m := m) leq T.WS
+      · apply e.IH; linarith
+    · case tapp m f T f.WS T.WS =>
+      constructor
+      · apply Var.WellScopedRec_weaken (m := m) leq f.WS
+      · apply Typ.WellScopedRec_weaken (m := m) leq T.WS
+    · case let_ m e1 e2 e1.WS e2.WS e1.IH e2.IH =>
+      constructor
+      · apply e1.IH leq
+      · apply e2.IH (n := n + 1); linarith
+    · case type m T e _ T.WS e.WS e.IH =>
+      constructor
+      · apply Typ.WellScopedRec_weaken (m := m) leq T.WS
+      · apply e.IH (n := n + 1); linarith
+    · case box m v _ v.WS =>
+      constructor
+      apply Var.WellScopedRec_weaken (m := m) leq v.WS
+    · case unbox m v _ v.WS =>
+      constructor
+      apply Var.WellScopedRec_weaken (m := m) leq v.WS
+
+  instance instWellScopedness : WellScopedness (Exp i) where
+    WellScopedRec := WellScopedRec
+    WellScoped := WellScoped
+    WellScoped_implies_WellScopedRec_0 := WellScoped_implies_WellScopedRec_0
+    WellScopedRec_weaken := WellScopedRec_weaken
+
+  @[aesop safe forward]
+  lemma substituteVar_fresh :
+    x ∉ freeVariablesVar e →
+    substituteVar e x u = e
+  := by induction e <;> aesop
+
+  @[aesop safe forward]
+  lemma instantiateRecVar_WellScopedRec :
+    WellScopedRec n e →
+    k >= n →
+    instantiateRecVar e k u = e
+  := by
+    intros WS geq
+    induction WS generalizing k <;> simp [instantiateRecVar]
+    · case var v v.WS =>
+      apply Var.instantiateRec_WellScopedRec v.WS geq
+    · case abs T e T.WS e.WS e.IH =>
+      aesop
+    · case app f e f.WS e.WS =>
+      apply And.intro
+        <;> apply Var.instantiateRec_WellScopedRec
+        <;> assumption
+    · case tabs T e T.WS e.WS e.IH =>
+      apply e.IH (k := k + 1); linarith
+    · case tapp f T f.WS T.WS =>
+      apply Var.instantiateRec_WellScopedRec <;> assumption
+    · case let_ e1 e2 e1.WS e2.WS e1.IH e2.IH =>
+      aesop
+    · case type T e T.WS e.WS e.IH =>
+      aesop
+    · case box v v.WS =>
+      apply Var.instantiateRec_WellScopedRec v.WS geq
+    · case unbox v v.WS =>
+      apply Var.instantiateRec_WellScopedRec v.WS geq
+
+  instance : Scoped (Exp i) (.var i) where
+    instantiateRec := instantiateRecVar
+    substitute := substituteVar
+    substitute_fresh := substituteVar_fresh
+    instantiateRec_WellScopedRec := instantiateRecVar_WellScopedRec
+    WellScopedRec_instantiateRec := WellScopedRec_instantiateRecVar
+
+  @[aesop safe forward]
+  lemma substituteTyp_fresh :
+    X ∉ freeVariablesTyp e →
+    substituteTyp e X U = e
+  := by
+    intros x.NotIn
+    induction e <;> simp [freeVariablesTyp] at x.NotIn <;> simp [substituteTyp]
+    · case abs T e e.IH =>
+      apply And.intro
+      . apply Typ.substituteTyp_fresh (by aesop)
+      · apply e.IH (by aesop)
+    · case tabs T e e.WS e.IH =>
+      apply And.intro
+      · apply Typ.substituteTyp_fresh (by aesop)
+      · apply e.IH (by aesop)
+    · case tapp f T =>
+      apply Typ.substituteTyp_fresh (by aesop)
+    · case let_ e1 e2 e1.IH e2.IH =>
+      apply And.intro
+      . apply e1.IH (by aesop)
+      · apply e2.IH (by aesop)
+    · case type T e T.WS e.WS e.IH =>
+      apply And.intro
+      · apply Typ.substituteTyp_fresh (by aesop)
+      · apply e.IH (by aesop)
+
+  @[aesop safe forward]
+  lemma instantiateRecTyp_WellScopedRec :
+    WellScopedRec n e →
+    k >= n →
+    instantiateRecTyp e k U = e
+  := by
+    intros WS geq
+    induction WS generalizing k <;> simp [instantiateRecTyp] <;> aesop
+
+  instance : Scoped (Exp i) (.tvar i) where
+    instantiateRec := instantiateRecTyp
+    substitute := substituteTyp
+    substitute_fresh := substituteTyp_fresh
+    WellScopedRec_instantiateRec := WellScopedRec_instantiateRecTyp
+    instantiateRec_WellScopedRec := instantiateRecTyp_WellScopedRec
+end Exp
