CCDeconstructed/Infrastructure/Typ.lean
@@ -1,0 +1,254 @@
+import CCDeconstructed.Syntax
+import CCDeconstructed.Classes
+import CCDeconstructed.Tactics
+import CCDeconstructed.Infrastructure.Var
+import CCDeconstructed.Infrastructure.Cap
+
+set_option linter.unusedVariables false
+
+open Scoped FreeVariables VarCat
+
+namespace Typ
+  instance : Coe (Var (.tvar i)) (Typ i) where
+    coe := Typ.var
+
+  @[aesop norm]
+  def freeVariablesTyp (T : Typ i) : Finset (Atom (.tvar i)) :=
+    match T with
+    | .top => ∅
+    | .var V => fv V
+    | .arr A B => A.freeVariablesTyp ∪ B.freeVariablesTyp
+    | .all _ A B => A.freeVariablesTyp ∪ B.freeVariablesTyp
+    | @Typ.box _ _ A => A.freeVariablesTyp
+    | .cap S _ => S.freeVariablesTyp
+
+  @[aesop norm]
+  def freeVariablesVar (T : Typ i) : Finset (Atom (.var i)) :=
+    match T with
+    | .top => ∅
+    | .var _ => ∅
+    | .arr A B => A.freeVariablesVar ∪ B.freeVariablesVar
+    | .all _ A B => A.freeVariablesVar ∪ B.freeVariablesVar
+    | @Typ.box _ _ A => A.freeVariablesVar
+    | .cap S C => S.freeVariablesVar ∪ fv C
+
+  instance instFreeVariablesVar : FreeVariables (Typ i) (.var i) where
+    fv := freeVariablesVar
+
+  instance instFreeVariablesTVar : FreeVariables (Typ i) (.tvar i) where
+    fv := freeVariablesTyp
+
+  @[aesop norm]
+  def instantiateRecTyp (T : Typ i) (K : Index (tvar i)) (U : Typ i) : Typ i :=
+    match T with
+    | .top => .top
+    | .var V => V.subst K U
+    | .arr A B => .arr (A.instantiateRecTyp K U) (B.instantiateRecTyp (K + 1) U)
+    | .all k A B => .all k (A.instantiateRecTyp K U) (B.instantiateRecTyp (K + 1) U)
+    | Typ.box A => .box (A.instantiateRecTyp K U)
+    | .cap S C => .cap (S.instantiateRecTyp K U) C
+
+  @[aesop norm]
+  def substituteTyp (T : Typ i) (X : Atom (.tvar i)) (U : Typ i) : Typ i :=
+    match T with
+    | .top => .top
+    | .var V => V.subst X U
+    | .arr A B => .arr (A.substituteTyp X U) (B.substituteTyp X U)
+    | .all k A B => .all k (A.substituteTyp X U) (B.substituteTyp X U)
+    | @Typ.box _ _ A => .box (A.substituteTyp X U)
+    | .cap S C => .cap (S.substituteTyp X U) C
+
+  @[aesop norm]
+  def instantiateRecVar (T : Typ i) (k : Index (.var i)) (u : Var (.var i)) : Typ i :=
+    match T with
+    | .top => .top
+    | .var V => V
+    | .arr A B => .arr (A.instantiateRecVar k u) (B.instantiateRecVar (k + 1) u)
+    | .all k' A B => .all k' (A.instantiateRecVar k u) (B.instantiateRecVar (k + 1) u)
+    | Typ.box A => .box (A.instantiateRecVar k u)
+    | .cap S C => .cap (S.instantiateRecVar k u) (C.instantiateRec k u)
+
+  @[aesop norm]
+  def substituteVar (T : Typ i) (x : Atom (.var i)) (u : Var (.var i)) : Typ i :=
+    match T with
+    | .top => .top
+    | .var V => V
+    | .arr A B => .arr (A.substituteVar x u) (B.substituteVar x u)
+    | .all k' A B => .all k' (A.substituteVar x u) (B.substituteVar x u)
+    | @Typ.box _ _ A => .box (A.substituteVar x u)
+    | .cap S C => .cap (S.substituteVar x u) (C.substitute x u)
+
+  @[aesop unsafe [constructors 50%]]
+  inductive WellScopedRec {i : CC} : Nat → Typ i → Prop :=
+    | top : WellScopedRec n .top
+    | var : Var.WellScopedRec (allowCap := false) n V → WellScopedRec n (.var V)
+    | arr :
+        WellScopedRec n A →
+        WellScopedRec (n + 1) B →
+        WellScopedRec n (.arr A B)
+    | all :
+        WellScopedRec n A →
+        WellScopedRec (n + 1) B →
+        WellScopedRec n (.all k A B)
+    | box [HasFeature i .box_type] :
+        WellScopedRec n T →
+        WellScopedRec n (.box T)
+    | cap :
+       WellScopedRec n S →
+       Cap.WellScopedRec n C →
+       WellScopedRec n (.cap S C)
+
+  @[aesop unsafe [constructors 50%]]
+  inductive WellScoped {i : CC} : Typ i → Prop :=
+    | top : WellScoped .top
+    | var : Var.WellScoped (allowCap := false) V → WellScoped (.var V)
+    | arr (L : Finset (Atom (.var i))) :
+        WellScoped T →
+        (∀ (x : Atom (.var i)), x ∉ L → WellScoped (U.instantiateRecVar 0 (.free x))) →
+        WellScoped (.arr T U)
+    | all (L : Finset (Atom (tvar i))) :
+        WellScoped S →
+        (∀ (X : Atom (.tvar i)), X ∉ L → WellScoped (U.instantiateRecTyp 0 (Typ.var X))) →
+        WellScoped (.all k S U)
+    | box [HasFeature i .box_type] :
+        WellScoped T →
+        WellScoped (.box T)
+    | cap :
+       WellScoped S →
+       WellScopedness.WellScoped C →
+       WellScoped (.cap S C)
+
+  @[aesop safe forward]
+  lemma WellScopedRec_instantiateRecTyp :
+    WellScopedRec n (instantiateRecTyp T n U) →
+    WellScopedRec (n + 1) T
+  := by
+    intros T.WS
+    generalize Eq : instantiateRecTyp T n U = T'
+    rw [Eq] at T.WS
+    induction' T.WS generalizing T
+    all_goals cases T
+      <;> simp only [instantiateRecTyp] at Eq
+      <;> constructor
+      <;> simp [Index] at *
+      <;> aesop
+    · linarith
+    . rename_i V K
+      suffices K < n_1 by simp [Index] at *; linarith
+      apply a_1 (.bound K) a_4
+
+  @[aesop safe forward]
+  lemma WellScopedRec_instantiateRecVar :
+    WellScopedRec n (instantiateRecVar T n u) →
+    WellScopedRec (n + 1) T
+  := by
+    intros T.WS
+    generalize Eq : instantiateRecVar T n u = T'
+    rw [Eq] at T.WS
+    induction' T.WS generalizing T
+    · case top n =>
+      cases T <;> simp only [instantiateRecVar] at Eq; constructor
+    · case var n V V.WS =>
+      cases T <;> simp only [instantiateRecVar] at Eq; constructor
+      apply Var.WellScopedRec_weaken (m := n) <;> aesop
+    · case arr =>
+      cases T <;> simp only [instantiateRecVar] at Eq; constructor <;> aesop
+    · case all =>
+      cases T <;> simp only [instantiateRecVar] at Eq; constructor <;> aesop
+    · case box =>
+      cases T <;> simp only [instantiateRecVar] at Eq; constructor; aesop
+    · case cap n S C S.WS C.WS S.IH =>
+      cases T <;> simp only [instantiateRecVar] at Eq
+      rename_i S' C'
+      injection Eq with Eq.S Eq.C
+      constructor
+      · apply S.IH; aesop
+      · apply Cap.WellScopedRec_instantiateRec (u := u)
+        rw [Eq.C]
+        exact C.WS
+
+  attribute [-aesop] specializeAnyScope
+  attribute [aesop unsafe tactic 80%] specializeAnyScope
+
+  @[aesop safe forward]
+  lemma WellScoped_implies_WellScopedRec_0 :
+    WellScoped T →
+    WellScopedRec 0 T
+  := by
+    intros WS
+    induction WS <;> constructor <;> aesop
+
+  @[aesop safe forward]
+  lemma WellScopedRec_weaken :
+    m <= n →
+    WellScopedRec m T →
+    WellScopedRec n T
+  := by
+    intros leq WS
+    induction' WS generalizing n <;> constructor <;> aesop
+    linarith
+
+  instance instWellScopedness : WellScopedness (Typ i) where
+    WellScopedRec := WellScopedRec
+    WellScoped := WellScoped
+    WellScoped_implies_WellScopedRec_0 := WellScoped_implies_WellScopedRec_0
+    WellScopedRec_weaken := WellScopedRec_weaken
+
+  @[aesop safe forward]
+  lemma substituteTyp_fresh :
+    X ∉ freeVariablesTyp T →
+    substituteTyp T X U = T
+  := by induction T <;> aesop
+
+  @[aesop safe forward]
+  lemma instantiateRecTyp_WellScopedRec :
+    WellScopedRec n T →
+    K >= n →
+    instantiateRecTyp T K U = T
+  := by
+    intros WS geq
+    induction WS generalizing K <;> aesop
+    exfalso; linarith
+
+  instance instScoped : Scoped (Typ i) (tvar i) where
+    instantiateRec := instantiateRecTyp
+    substitute := substituteTyp
+    substitute_fresh := substituteTyp_fresh
+    instantiateRec_WellScopedRec := instantiateRecTyp_WellScopedRec
+    WellScopedRec_instantiateRec := WellScopedRec_instantiateRecTyp
+
+  @[aesop safe forward]
+  lemma substituteVar_fresh :
+    x ∉ freeVariablesVar T →
+    substituteVar T x u = T
+  := by
+    intros x.NotIn
+    induction T <;> simp [substituteVar]
+    · case arr T U T.IH U.IH =>
+      apply And.intro <;> aesop
+    · case all S U S.IH U.IH =>
+      apply And.intro <;> aesop
+    · case box T T.IH =>
+      apply T.IH x.NotIn
+    · case cap S C S.IH =>
+      apply And.intro
+      · aesop
+      · apply Cap.substitute_fresh
+        aesop
+
+  @[aesop safe forward]
+  lemma instantiateRecVar_WellScopedRec :
+    WellScopedRec n T →
+    k >= n →
+    instantiateRecVar T k u = T
+  := by
+    intros WS geq
+    induction WS generalizing k <;> aesop
+
+  instance : Scoped (Typ i) (.var i) where
+    instantiateRec := instantiateRecVar
+    substitute := substituteVar
+    substitute_fresh := substituteVar_fresh
+    WellScopedRec_instantiateRec := WellScopedRec_instantiateRecVar
+    instantiateRec_WellScopedRec := instantiateRecVar_WellScopedRec
+end Typ
