CCDeconstructed/Infrastructure/Var.lean
@@ -1,0 +1,119 @@
+import CCDeconstructed.Syntax
+import CCDeconstructed.Classes
+
+open Scoped FreeVariables VarCat
+
+namespace Var
+  instance : Coe (Atom α) (Var α) where
+    coe := Var.free
+
+  instance : Coe (Index α) (Var α) where
+    coe := Var.bound
+
+  @[aesop norm]
+  def fv : Var α → Finset (Atom α)
+      | .free x => {x}
+      | .bound _ => ∅
+      | .cap => ∅
+
+  @[aesop norm]
+  def bv : Var α → Finset (Index α)
+    | .free _ => ∅
+    | .bound i => {i}
+    | .cap => ∅
+
+  @[simp,aesop norm]
+  def subst [Coe (Var α) β] (v : Var α) (x : Var α) (u : β) : β :=
+    if v = x then u else v
+
+  @[aesop norm]
+  def substitute {i} {α : VarCat i} (v : Var α) (x : Atom α) (u : Var α) : Var α :=
+    @subst i α (Var α) ⟨id⟩ v (.free x) u
+
+  @[aesop norm]
+  def instantiateRec {i} {α : VarCat i} (v : Var α) (k : Index α) (u : Var α) : Var α :=
+    @subst i α (Var α) ⟨id⟩ v (.bound k) u
+
+  instance instFreeVariables : FreeVariables (Var α) α where
+    fv := fv
+
+  @[aesop norm]
+  def WellScopedRec {i : CC} {α : VarCat i} (allowCap := false) (n : Nat) : Var α → Prop
+    | .bound k => k < n
+    | .free _ => True
+    | .cap => if allowCap then True else False
+
+  @[aesop norm]
+  def WellScoped {i : CC} {α : VarCat i} (allowCap := false) : Var α → Prop
+    | .bound _ => False
+    | .free _ => True
+    | .cap => if allowCap then True else False
+
+  @[aesop safe apply]
+  lemma WellScoped_implies_WellScopedRec_0 :
+    WellScoped allowCap t →
+    WellScopedRec allowCap 0 t
+  := by simp [WellScoped,WellScopedRec]
+
+  @[aesop safe apply]
+  lemma WellScopedRec_weaken :
+    m <= n →
+    WellScopedRec allowCap m v →
+    WellScopedRec allowCap n v
+  := by
+    simp [WellScopedRec]
+    intros
+    cases v
+    · case free => simp
+    · case bound => simp [Index] at *; linarith
+    · case cap => cases allowCap <;> simp at *
+
+  instance instWellScopedness (allowCap : Bool) : WellScopedness (Var α) where
+    WellScopedRec := WellScopedRec allowCap
+    WellScoped := WellScoped allowCap
+    WellScoped_implies_WellScopedRec_0 := WellScoped_implies_WellScopedRec_0
+    WellScopedRec_weaken := WellScopedRec_weaken
+
+  @[aesop safe apply]
+  lemma substitute_fresh :
+    x ∉ fv v →
+    substitute v x u = v
+  := by simp [fv,substitute]; aesop
+
+  @[aesop safe apply]
+  lemma WellScopedRec_instantiateRec :
+    WellScopedRec allowCap n (instantiateRec v n u)→
+    WellScopedRec allowCap (n + 1) v
+  := by
+    simp [WellScopedRec]
+    intros WS
+    cases v
+    · case free => simp
+    · case bound k =>
+      simp [instantiateRec] at *
+      cases (decEq k n) <;> rename_i H <;> simp [H,Index] at *
+      linarith
+    · case cap =>
+      simp [instantiateRec] at *
+      assumption
+
+  @[aesop safe apply]
+  lemma instantiateRec_WellScopedRec :
+    WellScopedRec allowCap n v →
+    k >= n →
+    instantiateRec v k u = v
+  := by
+    simp [instantiateRec,WellScopedRec]
+    intros WS leq v.Bound
+    cases v <;> simp [Index] at *
+    case bound k => exfalso; linarith
+
+  instance instScoped (allowCap : Bool) : Scoped (Var (.var i)) (.var i) where
+    instantiateRec := instantiateRec
+    substitute := substitute
+    substitute_fresh := substitute_fresh
+    WellScopedRec_instantiateRec := WellScopedRec_instantiateRec (allowCap := allowCap)
+    instantiateRec_WellScopedRec := instantiateRec_WellScopedRec (allowCap := allowCap)
+    WellScoped_implies_WellScopedRec_0 := WellScoped_implies_WellScopedRec_0
+    WellScopedRec_weaken := WellScopedRec_weaken
+end Var
