CCDeconstructed/Main.lean
@@ -1,8 +1,6 @@
-import CCDeconstructed.Atom
 import CCDeconstructed.CC
 import CCDeconstructed.Classes
 import CCDeconstructed.Env
-import CCDeconstructed.Index
 import CCDeconstructed.Infrastructure
 import CCDeconstructed.Syntax
 import CCDeconstructed.Tactics
