CCDeconstructed/Subcapturing.lean
@@ -1,0 +1,166 @@
+import CCDeconstructed.CC
+import CCDeconstructed.Var
+import CCDeconstructed.Syntax
+import CCDeconstructed.Classes
+import CCDeconstructed.Infrastructure
+import CCDeconstructed.WellFormedness
+
+open Feature VarCat
+
+variable {i : CC}
+
+inductive Cap.Sub (Γ : Env i) : Cap i → Cap i → Prop where
+  | elem :
+    Env.WellFormed Γ →
+    Cap.WellFormed Γ C →
+    Var.WellFormed (allowCap := true) Γ v →
+    v ∈ C →
+    Cap.Sub Γ {v} C
+  | set :
+    Env.WellFormed Γ →
+    Cap.WellFormed Γ D →
+    (∀ v ∈ C, Cap.Sub Γ {v} D) →
+    Cap.Sub Γ C D
+  | var :
+    Env.WellFormed Γ →
+    x ⦂ .cap S C ∈ Γ →
+    Cap.Sub Γ {.free x} C
+
+namespace Cap.Sub
+  lemma regular :
+    Sub Γ C D →
+    Env.WellFormed Γ ∧ WellFormed Γ C ∧ WellFormed Γ D
+  := by
+    intros Sub
+    induction Sub
+    · case elem C v Γ.WF C.WF v.WF v.In =>
+      apply And.intro Γ.WF
+      apply And.intro _ C.WF
+      intros w w.In
+      simp at w.In; cases w.In
+      exact v.WF
+    · case set D C Γ.WF D.WF Elem.Sub IH =>
+      apply And.intro Γ.WF (And.intro _ D.WF)
+      cases (Finset.eq_empty_or_nonempty C)
+      · case inl C.Empty =>
+        rw [C.Empty]
+        exact Cap.WellFormed_empty
+      · case inr C.Nonempty =>
+        obtain ⟨v, v.In⟩ := C.Nonempty
+
+  lemma empty :
+    Env.WellFormed Γ →
+    WellFormed Γ C →
+    Sub Γ ∅ C
+  := by
+    intros Γ.WF C.WF
+    apply Sub.set Γ.WF C.WF
+    simp
+
+  lemma WellFormed_in_empty_env_is_at_most_cap :
+    WellFormed ∅ C →
+    C ⊆ {@Var.cap i _ rfl}
+  := by
+    intros WF
+    intros v v.In
+    simp
+    simp [WellFormed] at WF
+    specialize WF v v.In
+    cases v <;> simp only [Var.WellFormed] at WF
+    · case free x =>
+      have : Env.dom (α := .var i) ∅ = ∅ := by
+        apply Env.dom_empty
+      simp [this] at WF
+    · case cap => rfl
+
+  lemma cap :
+    WellFormed (i := i) Γ C →
+    Sub (i := i) Γ C {@Var.cap i _ rfl}
+  := by
+    intros C.WF
+    induction Γ
+    · case empty =>
+      have C.AtMostCap := WellFormed_in_empty_env_is_at_most_cap C.WF
+      simp at C.AtMostCap
+      cases C.AtMostCap
+      · case inl C.Empty =>
+        rw [C.Empty]
+        apply set
+        intros v v.In
+        simp at v.In
+      · case inr C.IsCap =>
+        rw [C.IsCap]
+        apply elem
+        simp
+    · case val x T Γ x.NotIn IH =>
+      have : ∀ y ∈ C, Sub Γ {y} {.cap} :=
+        apply set
+      apply set
+
+      simp [WellFormed,Var.WellFormed,Env.dom,Finset.fold,List.foldr] at C.WF
+      cases C.decidableNonempty
+      · case isFalse h =>
+        simp at h
+        rw [h]
+        apply empty
+        intros v v.In
+        simp at v.In
+        rw [v.In]
+        constructor
+      · case isTrue h =>
+        obtain ⟨v, v.In⟩ := h
+        specialize C.WF v v.In
+        cases v <;> simp at C.WF
+        apply Sub.elem
+
+
+
+
+  lemma reflexivity :
+    Sub Γ C C
+  := by
+    apply Sub.set
+    intros x x.In
+    apply Sub.elem x.In
+
+  lemma distributivity :
+    Sub Γ C D →
+    ∀ v ∈ C, Sub Γ {v} D
+  := by
+    intros CD
+    cases CD
+    · case elem v v.In =>
+      intros w w.In
+      have Eq : v = w := by aesop
+      rw [<- Eq] at *
+      apply Sub.elem v.In
+    · case set Elem =>
+      exact Elem
+    · case var x S x.Bound =>
+      intros v v.In
+      cases v
+      · case free y =>
+        have Eq : x = y := by aesop
+        rw [<- Eq] at *
+        apply Sub.var x.Bound
+      · case bound k =>
+        exfalso; aesop
+      · case cap =>
+        exfalso; aesop
+
+  lemma transitivity C₂ :
+    Sub Γ C₁ C₂ →
+    Sub Γ C₂ C₃ →
+    Sub Γ C₁ C₃
+  := by
+    intros Sub₁₂ Sub₂₃
+    induction Sub₁₂
+    · case elem x C x.In =>
+      apply distributivity Sub₂₃ x x.In
+    · case set C₁ C₂ Elem IH =>
+      apply Sub.set
+      intros v v.In
+      apply IH v v.In Sub₂₃
+    · case var x S C₂ x.Bound =>
+      apply Sub.var
+end Cap.Sub
