lakefile.lean
@@ -6,5 +6,8 @@ package ccdeconstructed
 require mathlib from git
   "https://github.com/leanprover-community/mathlib4"@"v4.3.0-rc1"
 
+require quote4 from git
+  "https://github.com/leanprover-community/quote4"
+
 @[default_target]
 lean_lib CCDeconstructed
